examples/machine-code/hoare-triple/helperLib.sig
@@ -14,6 +14,7 @@ sig
     | FUN_COND of term * ftree_type
     | FUN_VAL of term;
 
+    val \\                     : tactic * tactic -> tactic
     val RW                     : thm list -> thm -> thm
     val RW1                    : thm list -> thm -> thm
 
@@ -81,6 +82,7 @@ sig
     val SEP_EXISTS_ELIM_RULE   : thm -> thm
     val SEP_EXISTS_POST_RULE   : term -> thm -> thm
     val SEP_EXISTS_PRE_RULE    : term -> thm -> thm
+    val SEP_REWRITE_RULE       : thm list -> thm -> thm
 
     val SPEC_STRENGTHEN_RULE   : thm -> term -> thm * term
     val SPEC_WEAKEN_RULE       : thm -> term -> thm * term
