examples/machine-code/compiler/compiler_demoScript.sml
@@ -118,6 +118,22 @@ val (thms,arm_str_rev_def,arm_str_rev_pre_def) = compile_all ``
       let r3 = r3 - 1w in
         arm_string_rev(r3,r6,r7,df,f)``
 
+(*
+
+val (th1,th2,th3) = compile
+
+
+val _ = arm_use_stack true;
+val target = "arm"
+val tm = ``
+  stack_loop (r1:word32,s4:word32,r5:word32) =
+    let r3 = s4 in
+    let s3 = r1 in
+      if r3 = 30w then (r1,r3,s3) else 
+        let r1 = r1 + r5 in 
+          stck_loop (r1,s4,r5)``;
+
+*)
 
 val _ = export_theory();
 
