examples/machine-code/garbage-collectors/improved_gcScript.sml
@@ -1,0 +1,1118 @@
+open HolKernel boolLib bossLib Parse; val _ = new_theory "improved_gc";
+
+open pred_setTheory arithmeticTheory pairTheory listTheory combinTheory;
+open finite_mapTheory sumTheory relationTheory;
+
+infix \\
+val op \\ = op THEN;
+val RW = REWRITE_RULE;
+val RW1 = ONCE_REWRITE_RULE;
+fun SUBGOAL q = REVERSE (q by ALL_TAC)
+fun ALPHA_TAC s = let
+  fun my_alpha_conv tm =
+    ALPHA_CONV (mk_var(s,type_of (fst(dest_abs tm)))) tm
+  in CONV_TAC (RAND_CONV my_alpha_conv) end;
+
+
+
+val _ = Hol_datatype `heap_address = H_ADDR of num | H_DATA of 'a`;
+val heap_address_11 = fetch "-" "heap_address_11";
+val heap_address_distinct = fetch "-" "heap_address_distinct";
+
+val _ = type_abbrev("abs_heap",``:(num |-> ('b heap_address) list # 'a) #
+          (num set) # (num set) # (num set) # (num -> num)``);
+
+val ADDR_MAP_def = Define `
+  (ADDR_MAP f [] = []) /\
+  (ADDR_MAP f (H_ADDR x::xs) = H_ADDR (f x) :: ADDR_MAP f xs) /\
+  (ADDR_MAP f (H_DATA y::xs) = H_DATA y :: ADDR_MAP f xs)`;
+
+val IN_THM = SIMP_RULE std_ss [EXTENSION,GSPECIFICATION]
+val ADDR_SET_def = (IN_THM o Define) `ADDR_SET s = { x | MEM (H_ADDR x) s }`;
+
+val (gc_reachable_rules,gc_reachable_ind,gc_reachable_cases) = Hol_reln `
+  (!h roots x.
+    x IN ADDR_SET roots ==> gc_reachable (h,roots) x) /\
+  (!h roots x a xs d.
+    a IN FDOM h /\ (h ' a = (xs,d)) /\ x IN ADDR_SET xs /\ gc_reachable (h,roots) a ==>
+    gc_reachable (h,roots) x)`;
+
+val PAIR_TRANSLATE_def = Define `PAIR_TRANSLATE f (xs,a) = (ADDR_MAP f xs,a)`;  
+val SET_TRANSLATE_def = (IN_THM o Define) `SET_TRANSLATE f s = { x | (f x) IN s }`;
+val HAS_CHANGED_def = (IN_THM o Define) `HAS_CHANGED f = { x | ~(f x = x) }`;
+val POINTERS_def = (IN_THM o Define) `POINTERS h y =
+  { a | ?b zs d. b IN y /\ b IN FDOM h /\ (h ' b = (zs,d)) /\ a IN ADDR_SET zs }`;
+
+val gc_filter_def = Define `
+  gc_filter (h,roots) = (DRESTRICT h (gc_reachable (h,roots)),roots)`; 
+
+val gc_copy_def = Define `
+  gc_copy (h1,roots1) (h2,roots2) = 
+    ?f. (f o f = I) /\ (FDOM h1 = SET_TRANSLATE f (FDOM h2)) /\
+        (roots2 = ADDR_MAP f roots1) /\
+        !x. x IN FDOM h1 ==> (h1 ' x = PAIR_TRANSLATE f (h2 ' (f x)))`;
+
+val gc_exec_def = Define `gc_exec x y = gc_copy (gc_filter x) y`;
+
+val (abs_step_rules,abs_step_ind,abs_step_cases) = Hol_reln `
+  (!h x y z f a.
+    a IN z /\ ~(f a = a) ==>
+    abs_step (h,x,y,z,f) (h,x,y,z DELETE a,f)) /\
+  (!h x y z f a xs d.
+    a IN y /\ (h ' a = (xs,d)) /\ (!b. b IN ADDR_SET xs ==> ~(f b = b)) ==>
+    abs_step (h,x,y,z,f) (h |+ (a,ADDR_MAP f xs,d),a INSERT x,y DELETE a,z,f)) /\
+  (!h x y z f a b xs d.
+    a IN z /\ (f a = a) /\ (f b = b) /\ ~(b IN FDOM h) /\ a IN FDOM h /\ (h ' a = (xs,d)) ==>
+    abs_step (h,x,y,z,f) (h |+ (b,xs,d) \\ a,x,b INSERT y,z UNION (ADDR_SET xs),(a =+ b) ((b =+ a) f)))`;
+
+val abs_steps_def = Define `abs_steps = RTC abs_step`;
+
+val abs_steps_TRANS = store_thm("abs_steps_TRANS",
+  ``!x y z. abs_steps x y /\ abs_steps y z ==> abs_steps x z``,
+  METIS_TAC [abs_steps_def,RTC_RTC]);
+
+val (abs_gc_rules,abs_gc_ind,abs_gc_cases) = Hol_reln `
+  (!h roots h2 f x.
+    abs_steps (h,{},{},ADDR_SET roots,I) (h2,x,{},{},f) ==>
+    abs_gc (h,roots) (DRESTRICT h2 x,ADDR_MAP f roots))`;
+
+val abs_gc_inv_def = Define `
+  abs_gc_inv (h1,roots1) (h,x,y,z,f) =
+    let old = FDOM h UNION HAS_CHANGED f DIFF (x UNION y) in
+      DISJOINT x y /\ 
+      POINTERS h x SUBSET (x UNION y) /\ 
+      POINTERS h (UNIV DIFF x) SUBSET old /\
+      POINTERS h y UNION ADDR_SET roots1 SUBSET SET_TRANSLATE f (x UNION y) UNION z /\
+      SET_TRANSLATE f (x UNION y) UNION z SUBSET gc_reachable (h1,roots1) /\
+      (!a. a IN z ==> if f a = a then a IN old else f a IN x UNION y) /\
+      (!a. ~(f a = a) ==> ~(a IN x UNION y = f a IN x UNION y)) /\   
+      (!a. a IN y \/ a IN x = ~(f a = a) /\ a IN FDOM h) /\ (f o f = I) /\ 
+      (SET_TRANSLATE f (FDOM h) = FDOM h1) /\
+      (!d. d IN FDOM h1 ==> 
+          (h1 ' d = if (f d) IN x then PAIR_TRANSLATE f (h ' (f d)) else h ' (f d)))`;
+
+val SET_TAC = 
+  FULL_SIMP_TAC std_ss [EXTENSION,IN_INSERT,IN_UNION,IN_DELETE,SUBSET_DEF,
+    DISJOINT_DEF,NOT_IN_EMPTY,EXTENSION,IN_INSERT,IN_INTER,IN_DIFF,IN_UNIV]
+  \\ METIS_TAC [PAIR_EQ];
+
+val SET2_TAC = 
+  FULL_SIMP_TAC std_ss [EXTENSION,IN_INSERT,IN_UNION,IN_DELETE,SUBSET_DEF,
+    DISJOINT_DEF,NOT_IN_EMPTY,EXTENSION,IN_INSERT,IN_INTER,IN_DIFF,IN_UNIV,
+    IN_LIST_TO_SET,POINTERS_def,HAS_CHANGED_def,SET_TRANSLATE_def,FDOM_FUPDATE,
+    FDOM_DOMSUB,FAPPLY_FUPDATE_THM,DOMSUB_FAPPLY_THM] \\ SET_TAC;
+
+val POINTERS_IGNORE = prove(
+  ``~(a IN x) ==> (POINTERS (h |+ (a,xs,d)) x = POINTERS h x) /\
+                  (POINTERS (h \\ a) x = POINTERS h x)``,
+  SET2_TAC);
+
+val set_SUBSET_POINTERS = prove(
+  ``(h ' a = (xs,d)) /\ a IN FDOM h /\ a IN x ==> ADDR_SET xs SUBSET POINTERS h x``,
+  SET2_TAC);
+
+val POINTER_FUPDATE_EQ = prove(
+  ``~(b IN FDOM h) /\ b IN x ==>
+    (POINTERS (h |+ (b,xs,d)) x = POINTERS h x UNION ADDR_SET xs)``,
+  SET2_TAC);
+
+val POINTERS_FUPDATE = prove(
+  ``POINTERS (h |+ (b,xs,d)) (b INSERT y) SUBSET POINTERS h y UNION ADDR_SET xs``,
+  SET2_TAC);
+
+val POINTERS_SUBSET = prove(
+  ``!h x y. x SUBSET y ==> POINTERS h x SUBSET POINTERS h y``,
+  SET2_TAC);
+  
+val POINTERS_DOMSUB = prove(
+  ``!h y. POINTERS (h \\ a) y SUBSET POINTERS h y``,
+  SET2_TAC);
+
+val SET_TRANSLATE_SUBSET = prove(
+  ``!f x y. (f o f = I) ==>
+            (SET_TRANSLATE f x SUBSET y = x SUBSET SET_TRANSLATE f y)``,
+  SIMP_TAC std_ss [FUN_EQ_THM] \\ SET2_TAC);
+
+val SET_TRANSLATE_MAP = prove(
+  ``!xs f. (f o f = I) ==> (ADDR_SET (ADDR_MAP f xs) = SET_TRANSLATE f (ADDR_SET xs))``,
+  SIMP_TAC std_ss [EXTENSION,ADDR_SET_def,SET_TRANSLATE_def]
+  \\ FULL_SIMP_TAC std_ss [FUN_EQ_THM] \\ Induct
+  \\ ASM_SIMP_TAC std_ss [ADDR_MAP_def,MEM] \\ Cases 
+  \\ ASM_SIMP_TAC std_ss [ADDR_MAP_def,MEM,heap_address_11,heap_address_distinct]
+  \\ SET2_TAC);
+
+val SET_TRANSLATE_THM = prove(
+  ``(f o f = I) ==> 
+     (SET_TRANSLATE f (x UNION y) = (SET_TRANSLATE f x) UNION (SET_TRANSLATE f y)) /\
+     (SET_TRANSLATE f (x INTER y) = (SET_TRANSLATE f x) INTER (SET_TRANSLATE f y)) /\
+     (SET_TRANSLATE f (a INSERT x) = (f a) INSERT (SET_TRANSLATE f x)) /\
+     (SET_TRANSLATE f (SET_TRANSLATE f x) = x)``,
+  SIMP_TAC std_ss [EXTENSION] \\ SIMP_TAC std_ss [FUN_EQ_THM] \\ SET2_TAC);
+
+val SET_TRANSLATE_IGNORE = prove(
+  ``(f o f = I) /\ (f a = a) /\ (f b = b) /\ ~(a IN x) /\ ~(b IN x) ==> 
+      (SET_TRANSLATE ((a =+ b) ((b =+ a) f)) x = SET_TRANSLATE f x)``,
+  SIMP_TAC std_ss [EXTENSION] \\ SIMP_TAC std_ss [FUN_EQ_THM,APPLY_UPDATE_THM,
+    SET_TRANSLATE_def] \\ SET2_TAC);
+
+val ADDR_MAP_ADDR_MAP = prove(
+  ``!xs f. (f o f = I) ==> (ADDR_MAP f (ADDR_MAP f xs) = xs)``,
+  Induct \\ SIMP_TAC std_ss [ADDR_MAP_def] \\ Cases
+  \\ ASM_SIMP_TAC std_ss [ADDR_MAP_def,FUN_EQ_THM]); 
+
+val ADDR_MAP_EQ_ADDR_MAP = prove(
+  ``!xs f g. (ADDR_MAP f xs = ADDR_MAP g xs) = !x. x IN ADDR_SET xs ==> (f x = g x)``,
+  Induct \\ SIMP_TAC std_ss [ADDR_MAP_def,ADDR_SET_def,MEM] 
+  \\ Cases \\ FULL_SIMP_TAC std_ss [ADDR_MAP_def,ADDR_SET_def,MEM,CONS_11,
+       heap_address_11,heap_address_distinct] \\ SET_TAC);
+
+val abs_step_thm = prove(
+  ``!s1 s2. abs_step s1 s2 /\ abs_gc_inv (h0,r0) s1 ==> abs_gc_inv (h0,r0) s2``,
+  REPEAT STRIP_TAC \\ Q.PAT_ASSUM `abs_step s1 s1i` ASSUME_TAC
+  \\ FULL_SIMP_TAC std_ss [abs_step_cases]
+  THEN1 (FULL_SIMP_TAC std_ss [abs_gc_inv_def,IN_UNION,IN_DELETE,LET_DEF]
+         \\ `f a IN x UNION y` by SET_TAC
+         \\ SUBGOAL `a IN SET_TRANSLATE f (x UNION y)` THEN1 SET_TAC \\ SET2_TAC)
+  THEN1
+   (FULL_SIMP_TAC std_ss [abs_gc_inv_def,IN_UNION,IN_DELETE,FDOM_FUPDATE,LET_DEF]
+    \\ `a INSERT FDOM h = FDOM h` by SET_TAC \\ ASM_SIMP_TAC std_ss [IN_INSERT]
+    \\ `~(a IN x) /\ ~(a IN (FDOM h UNION HAS_CHANGED f DIFF (a INSERT x)))` by SET_TAC 
+    \\ ASM_SIMP_TAC std_ss [POINTERS_IGNORE] \\ STRIP_TAC THEN1 SET_TAC
+    \\ `(a INSERT x) UNION (y DELETE a) UNION z = x UNION y UNION z` by SET_TAC
+    \\ `(a INSERT x) UNION (y DELETE a) = x UNION y` by SET_TAC
+    \\ ASM_SIMP_TAC std_ss []
+    \\ REVERSE (REPEAT STRIP_TAC) THEN1
+     (Cases_on `f d' = a` \\ ASM_SIMP_TAC std_ss [FAPPLY_FUPDATE_THM,IN_INSERT]
+      \\ `~(a IN x)` by SET_TAC 
+      \\ ASM_SIMP_TAC std_ss [PAIR_TRANSLATE_def,ADDR_MAP_ADDR_MAP])
+    THEN1 SET_TAC THEN1 SET_TAC THEN1 SET_TAC THEN1 SET2_TAC THEN1 SET2_TAC
+    \\ MATCH_MP_TAC (MATCH_MP (RW [GSYM AND_IMP_INTRO] SUBSET_TRANS) (SPEC_ALL POINTERS_FUPDATE))
+    \\ ASM_SIMP_TAC std_ss [UNION_SUBSET] \\ `a IN FDOM h` by SET_TAC
+    \\ IMP_RES_TAC set_SUBSET_POINTERS \\ POP_ASSUM (K ALL_TAC)
+    \\ ASM_SIMP_TAC std_ss [SET_TRANSLATE_MAP,SET_TRANSLATE_SUBSET] \\ SET2_TAC)
+  THEN1   
+   (FULL_SIMP_TAC std_ss [abs_gc_inv_def,IN_UNION,IN_DELETE,FDOM_FUPDATE,IN_INSERT,LET_DEF]
+    \\ `~(a IN x) /\ ~(b IN x) /\ ~(a = b) /\ a IN (UNIV DIFF x) /\ a IN (UNIV DIFF (x UNION y))` by SET_TAC 
+    \\ `ADDR_SET xs SUBSET POINTERS h (U(:num) DIFF (x UNION y))` by METIS_TAC [set_SUBSET_POINTERS]
+    \\ `((a =+ b) ((b =+ a) f) o (a =+ b) ((b =+ a) f) = I)` by 
+         (FULL_SIMP_TAC std_ss [APPLY_UPDATE_THM,FUN_EQ_THM] \\ SET_TAC)
+    \\ STRIP_TAC THEN1 SET_TAC
+    \\ ASM_SIMP_TAC std_ss [POINTERS_IGNORE] \\ STRIP_TAC THEN1 SET_TAC
+    \\ `(HAS_CHANGED ((a =+ b) ((b =+ a) f)) = a INSERT b INSERT HAS_CHANGED f) /\
+       ~(b IN HAS_CHANGED f)` by 
+        (FULL_SIMP_TAC std_ss [EXTENSION,HAS_CHANGED_def,APPLY_UPDATE_THM] \\ SET2_TAC)
+    \\ STRIP_TAC THEN1 (FULL_SIMP_TAC std_ss [] \\ SET2_TAC)
+    \\ `~(a IN y) /\ ~(b IN y)` by SET_TAC
+    \\ FULL_SIMP_TAC std_ss [SET_TRANSLATE_THM,APPLY_UPDATE_THM,SET_TRANSLATE_IGNORE]
+    \\ STRIP_TAC THEN1 SET2_TAC
+    \\ STRIP_TAC THEN1
+     (`a IN gc_reachable (h0,r0)` by SET_TAC
+      \\ SUBGOAL `ADDR_SET xs SUBSET gc_reachable (h0,r0)` THEN1 SET_TAC
+      \\ FULL_SIMP_TAC std_ss [SUBSET_DEF] \\ REPEAT STRIP_TAC
+      \\ SIMP_TAC std_ss [IN_DEF] \\ ONCE_REWRITE_TAC [gc_reachable_cases]
+      \\ DISJ2_TAC \\ Q.PAT_ASSUM `a IN gc_reachable hhh` 
+           (ASSUME_TAC o SIMP_RULE std_ss [IN_DEF]) \\ ASM_SIMP_TAC std_ss []
+      \\ Q.LIST_EXISTS_TAC [`a`,`xs`,`d`] \\ ASM_SIMP_TAC std_ss [] \\ SET2_TAC)
+    \\ STRIP_TAC THEN1
+     (FULL_SIMP_TAC std_ss [FDOM_FUPDATE,FDOM_DOMSUB]
+      \\ ALPHA_TAC "n" \\ REPEAT STRIP_TAC THEN1
+       (Cases_on `a = n` \\ FULL_SIMP_TAC std_ss []
+        \\ SUBGOAL `~(n = b)` THEN1 (FULL_SIMP_TAC std_ss [FUN_EQ_THM] \\ SET_TAC)
+        \\ CCONTR_TAC \\ FULL_SIMP_TAC std_ss []
+        \\ `~(b IN HAS_CHANGED f)` by (SIMP_TAC std_ss [HAS_CHANGED_def] \\ SET_TAC)
+        \\ SET_TAC)
+      \\ Cases_on `a = n` \\ FULL_SIMP_TAC std_ss [] 
+      \\ `POINTERS h (U(:num) DIFF (x UNION y)) SUBSET POINTERS h (U(:num) DIFF x)` by 
+           (MATCH_MP_TAC POINTERS_SUBSET \\ SET_TAC) 
+      \\ `n IN FDOM h UNION HAS_CHANGED f DIFF (x UNION y)` by SET_TAC
+      \\ FULL_SIMP_TAC std_ss [IN_INSERT,IN_UNION,IN_DELETE,IN_DIFF] \\ SET_TAC)
+    \\ FULL_SIMP_TAC std_ss [FDOM_DOMSUB,FDOM_FUPDATE,IN_INSERT]
+    \\ STRIP_TAC THEN1 (FULL_SIMP_TAC std_ss [FUN_EQ_THM] \\ SET_TAC)
+    \\ STRIP_TAC THEN1 (FULL_SIMP_TAC std_ss [FUN_EQ_THM] \\ SET_TAC)
+    \\ Q.PAT_ASSUM `gg = FDOM h0` (ASSUME_TAC o GSYM) \\ ASM_SIMP_TAC std_ss []
+    \\ STRIP_TAC THEN1
+     (FULL_SIMP_TAC std_ss [EXTENSION,SET_TRANSLATE_def,APPLY_UPDATE_THM]
+      \\ FULL_SIMP_TAC std_ss [FUN_EQ_THM] \\ SET_TAC)
+    \\ ALPHA_TAC "i" \\ STRIP_TAC
+    \\ Cases_on `(i = a) \/ (i = b)` \\ FULL_SIMP_TAC std_ss [APPLY_UPDATE_THM,
+        FUN_EQ_THM,DOMSUB_FAPPLY_THM,FAPPLY_FUPDATE_THM]
+    THEN1 (FULL_SIMP_TAC std_ss [SET_TRANSLATE_def])
+    \\ `~(f i = a) /\ ~(f i = b)` by METIS_TAC []
+    \\ Cases_on `f i IN x` \\ FULL_SIMP_TAC std_ss []
+    \\ `?xs d. h ' (f i) = (xs,d)` by METIS_TAC [PAIR]
+    \\ ASM_SIMP_TAC std_ss [PAIR_TRANSLATE_def,IN_DEF,SET_TRANSLATE_def]
+    \\ ASM_SIMP_TAC std_ss [ADDR_MAP_EQ_ADDR_MAP,APPLY_UPDATE_THM]
+    \\ REPEAT STRIP_TAC
+    \\ `ADDR_SET xs' SUBSET x UNION y` by METIS_TAC [set_SUBSET_POINTERS,SUBSET_TRANS]
+    \\ SET_TAC));
+
+val abs_steps_thm = prove(
+  ``!s1 s2. abs_steps s1 s2 /\ abs_gc_inv (h0,r0) s1 ==> abs_gc_inv (h0,r0) s2``,
+  SIMP_TAC std_ss [GSYM AND_IMP_INTRO,abs_steps_def] 
+  \\ HO_MATCH_MP_TAC RTC_INDUCT \\ SIMP_TAC std_ss [] \\ METIS_TAC [abs_step_thm]);
+
+val ok_heap_def = Define `
+  ok_heap (h,roots) = (POINTERS h UNIV UNION ADDR_SET roots SUBSET FDOM h)`;
+
+val ok_heap_IMP = store_thm("ok_heap_IMP",
+  ``ok_heap (h1,roots1) ==> abs_gc_inv (h1,roots1) (h1,{},{},ADDR_SET roots1,I)``,
+  FULL_SIMP_TAC std_ss [abs_gc_inv_def,LET_DEF,ok_heap_def] 
+  \\ SUBGOAL `ADDR_SET roots1 SUBSET gc_reachable (h1,roots1)` THEN1 SET2_TAC
+  \\ SIMP_TAC std_ss [SUBSET_DEF] \\ REPEAT STRIP_TAC \\ SIMP_TAC std_ss [IN_DEF] 
+  \\ ONCE_REWRITE_TAC [gc_reachable_cases] \\ ASM_SIMP_TAC std_ss []);
+
+val abs_gc_thm = store_thm("abs_gc_thm",
+  ``!h1 roots1 h2 roots2.
+       ok_heap (h1,roots1) /\ abs_gc (h1,roots1) (h2,roots2) ==> 
+       gc_exec (h1,roots1) (h2,roots2)``,
+  SIMP_TAC std_ss [abs_gc_cases,gc_exec_def,gc_filter_def,gc_copy_def] 
+  \\ REPEAT STRIP_TAC \\ Q.EXISTS_TAC `f` \\ ASM_SIMP_TAC std_ss []
+  \\ IMP_RES_TAC ok_heap_IMP \\ IMP_RES_TAC abs_steps_thm \\ POP_ASSUM MP_TAC 
+  \\ SIMP_TAC std_ss [abs_gc_inv_def,LET_DEF,NOT_IN_EMPTY,UNION_EMPTY]
+  \\ STRIP_TAC \\ SIMP_TAC std_ss [FDOM_DRESTRICT,DRESTRICT_DEF]
+  \\ SUBGOAL `gc_reachable (h1,roots1) = SET_TRANSLATE f x` THEN1 SET2_TAC
+  \\ ASM_SIMP_TAC std_ss [SET_EQ_SUBSET] \\ SIMP_TAC std_ss [SUBSET_DEF] 
+  \\ `?tt. (h1,roots1) = tt` by METIS_TAC [PAIR] \\ ASM_SIMP_TAC std_ss []
+  \\ REPEAT STRIP_TAC \\ REPEAT (POP_ASSUM MP_TAC) 
+  \\ SIMP_TAC std_ss [AND_IMP_INTRO] \\ ONCE_REWRITE_TAC [CONJ_COMM]
+  \\ SIMP_TAC std_ss [GSYM CONJ_ASSOC] \\ SIMP_TAC std_ss [GSYM AND_IMP_INTRO]
+  \\ STRIP_TAC \\ POP_ASSUM (MP_TAC o SIMP_RULE std_ss [IN_DEF])
+  \\ Q.SPEC_TAC (`x'`,`q`) \\ Q.SPEC_TAC (`tt`,`t`) 
+  \\ HO_MATCH_MP_TAC gc_reachable_ind \\ REPEAT STRIP_TAC THEN1 SET_TAC   
+  \\ FULL_SIMP_TAC std_ss [SET_TRANSLATE_def] 
+  \\ `h2' ' (f q') = (ADDR_MAP f xs,d)` by ALL_TAC THEN1
+    (Q.PAT_ASSUM `!d. d IN FDOM h ==> bb` (MP_TAC o GSYM o Q.SPEC `q'`)       
+     \\ `?xs2 d2. h2' ' (f q') = (xs2,d2)` by METIS_TAC [PAIR]
+     \\ ASM_SIMP_TAC std_ss [PAIR_TRANSLATE_def] 
+     \\ ONCE_REWRITE_TAC [EQ_SYM_EQ] 
+     \\ ASM_SIMP_TAC std_ss [ADDR_MAP_ADDR_MAP])
+  \\ `ADDR_SET (ADDR_MAP f xs) SUBSET POINTERS h2' x` by METIS_TAC [set_SUBSET_POINTERS]
+  \\ `f q IN ADDR_SET (ADDR_MAP f xs)` by ALL_TAC THEN1
+      (FULL_SIMP_TAC std_ss [SET_TRANSLATE_MAP,SET_TRANSLATE_def]
+       \\ FULL_SIMP_TAC std_ss [FUN_EQ_THM]) \\ SET_TAC);
+
+val gc_copy_thm = prove(
+  ``ok_heap (h1,roots1) /\ gc_copy (h1,roots1) (h2,roots2) ==> ok_heap (h2,roots2)``,
+  SIMP_TAC std_ss [gc_exec_def,gc_copy_def,gc_filter_def,ok_heap_def]
+  \\ REPEAT STRIP_TAC \\ FULL_SIMP_TAC std_ss [SUBSET_DEF,IN_UNION,POINTERS_def]
+  \\ `!k. f (f k) = k` by FULL_SIMP_TAC std_ss [FUN_EQ_THM]
+  \\ REVERSE (REPEAT STRIP_TAC) THEN1
+   (POP_ASSUM MP_TAC \\ FULL_SIMP_TAC std_ss [SET_TRANSLATE_MAP,SET_TRANSLATE_def]  
+    \\ SET_TAC)
+  \\ FULL_SIMP_TAC std_ss [IN_UNIV,SET_TRANSLATE_def,EXTENSION]  
+  \\ Q.PAT_ASSUM `!d. ff IN FDOM h1 <=> bb IN FDOM h2` ASSUME_TAC
+  \\ FULL_SIMP_TAC std_ss [] 
+  \\ `h1 ' (f b) = PAIR_TRANSLATE f (zs,d)` by METIS_TAC []
+  \\ FULL_SIMP_TAC std_ss [PAIR_TRANSLATE_def]
+  \\ SUBGOAL `f x IN ADDR_SET (ADDR_MAP f zs)` THEN1 METIS_TAC []
+  \\ FULL_SIMP_TAC std_ss [SET_TRANSLATE_MAP,SET_TRANSLATE_def]);
+
+val gc_filter_thm = prove(
+  ``ok_heap (h1,roots1) ==> ok_heap (gc_filter(h1,roots1))``,
+  SIMP_TAC std_ss [gc_exec_def,gc_copy_def,gc_filter_def,ok_heap_def]
+  \\ REPEAT STRIP_TAC \\ FULL_SIMP_TAC std_ss [SUBSET_DEF,IN_UNION,POINTERS_def]
+  \\ REVERSE (REPEAT STRIP_TAC) THEN1
+   (RES_TAC \\ FULL_SIMP_TAC std_ss [FDOM_DRESTRICT,IN_INTER]     
+    \\ FULL_SIMP_TAC std_ss [IN_DEF] \\ ONCE_REWRITE_TAC [gc_reachable_cases]
+    \\ ASM_SIMP_TAC std_ss [IN_DEF])
+  \\ FULL_SIMP_TAC std_ss [FDOM_DRESTRICT,IN_INTER]
+  \\ Q.PAT_ASSUM `DRESTRICT h1 (gc_reachable (h1,roots1)) ' b = (zs,d)` MP_TAC
+  \\ ASM_SIMP_TAC std_ss [DRESTRICT_DEF,IN_INTER] \\ REPEAT STRIP_TAC THEN1 SET_TAC
+  \\ FULL_SIMP_TAC std_ss [IN_DEF]
+  \\ ONCE_REWRITE_TAC [gc_reachable_cases] \\ DISJ2_TAC
+  \\ SIMP_TAC std_ss [] \\ Q.EXISTS_TAC `b` \\ ASM_SIMP_TAC std_ss [IN_DEF]);
+
+val gc_exec_thm = store_thm("gc_exec_thm",
+  ``ok_heap (h1,roots1) /\ gc_exec (h1,roots1) (h2,roots2) ==> ok_heap (h2,roots2)``,
+  METIS_TAC [gc_exec_def,gc_filter_thm,gc_copy_thm,PAIR]);
+
+(* next level *)
+
+val _ = Hol_datatype `heap_element =
+    H_EMP | H_REF of num | H_BLOCK of ('a heap_address) list # (num # 'b)`;
+val heap_element_distinct = fetch "-" "heap_element_distinct";
+val heap_element_11 = fetch "-" "heap_element_11";
+
+val isDATA_def = Define `isDATA x = ?i. x = H_DATA i`;
+val isADDR_def = Define `isADDR x = ?i. x = H_ADDR i`;
+val isREF_def = Define `isREF x = ?i. x = H_REF i`;
+val isBLOCK_def = Define `isBLOCK x = ?i. x = H_BLOCK i`;
+val getADDR_def = Define `getADDR (H_ADDR x) = x`;
+val getREF_def = Define `getREF (H_REF x) = x`;
+val getBLOCK_def = Define `getBLOCK (H_BLOCK y) = y`;
+val getLENGTH_def = Define `
+  (getLENGTH (H_BLOCK (m,l,n)) = l + 1) /\
+  (getLENGTH (H_REF i) = 0) /\
+  (getLENGTH (H_EMP) = 0)`;
+
+val RANGE_def = Define `RANGE(i:num,j) k = i <= k /\ k < j`;
+val CUT_def = Define `CUT (i,j) m = \k. if RANGE (i,j) k then m k else H_EMP`;
+
+val D0 = Define `D0 m k = ?x y z. m (k:num) = H_BLOCK (x,y,z)`;
+val D1 = Define `D1 m i = ?k x y z. (m (k:num) = H_BLOCK(x,y,z)) /\ i IN ADDR_SET x`;
+val R0 = Define `R0 m k = ?a. m (k:num) = H_REF a`;
+val R1 = Define `R1 m a = ?k. m (k:num) = H_REF a`;
+val DR0 = Define `DR0 m k = D0 m k \/ R0 m k`
+val DR1 = Define `DR1 m k = D1 m k \/ R1 m k`
+
+val move_def = Define `
+  (move (H_DATA x,j,m) = (H_DATA x,j,m)) /\
+  (move (H_ADDR a,j,m) =
+     case m a of
+        H_REF i -> (H_ADDR i,j,m)
+     || H_BLOCK (xs,n,d) -> let m = (a =+ H_REF j) m in
+                            let m = (j =+ H_BLOCK (xs,n,d)) m in
+                              (H_ADDR j,j + n + 1,m))`;
+
+val move_list_def = Define `
+  (move_list ([],j,m) = ([],j,m)) /\
+  (move_list (x::xs,j,m) =
+     let (x,j,m) = move (x,j,m) in
+     let (xs,j,m) = move_list (xs,j,m) in
+       (x::xs,j,m))`;
+
+val gc_step_def = Define `
+  gc_step (i,j,m) = 
+    let (xs,n,d) = getBLOCK (m i) in
+    let (xs,j,m) = move_list (xs,j,m) in
+    let m = (i =+ H_BLOCK (xs,n,d)) m in
+    let i = i + n + 1 in
+      (i,j,m)`; 
+
+val (gc_loop_def,_) = tailrecLib.tailrec_define ``
+  gc_loop (i,j,m) = if i = j then (i,m) else
+                      let (i,j,m) = gc_step (i,j,m) in
+                        gc_loop (i,j,m)`` NONE
+
+val gc_def = Define `
+  gc (b:num,e:num,b2:num,e2:num,roots,m) =
+    let (b2,e2,b,e) = (b,e,b2,e2) in
+    let (roots,j,m) = move_list (roots,b,m) in
+    let (i,m) = gc_loop (b,j,m) in
+    let m = CUT (b,i) m in
+      (b,i,e,b2,e2,roots,m)`;
+
+(* invariant *)
+
+val EMP_RANGE_def = Define `
+  EMP_RANGE (b,e) m = !k. k IN RANGE(b,e) ==> (m k = H_EMP)`;
+
+val (full_heap_rules,full_heap_ind,full_heap_cases) =
+  Hol_reln
+  `(!b m. full_heap b b m) /\
+   (!b e m n xs d.
+      (m b = H_BLOCK (xs,n,d)) /\ EMP_RANGE (b+1,b+n+1) m /\
+      full_heap (b+n+1) e m ==> full_heap b e m)`;
+
+val full_heap_ind = IndDefLib.derive_strong_induction(full_heap_rules,full_heap_ind);
+val _ = save_thm("full_heap_ind",full_heap_ind);
+
+val (part_heap_rules,part_heap_ind,part_heap_cases) =
+  Hol_reln
+  `(!b m. part_heap b b m 0) /\
+   (!b e m k. 
+      ~(isBLOCK (m b)) /\ part_heap (b+1) e m k ==> part_heap b e m k) /\
+   (!b e m n xs d k.
+      (m b = H_BLOCK (xs,n,d)) /\ EMP_RANGE (b+1,b+n+1) m /\
+      part_heap (b+n+1) e m k ==> part_heap b e m (k+n+1))`;
+   
+val part_heap_ind = IndDefLib.derive_strong_induction(part_heap_rules,part_heap_ind);
+val _ = save_thm("part_heap_ind",part_heap_ind);
+
+val ref_mem_def = Define `
+  ref_mem (h,f) m = 
+    !a. m a = if a IN FDOM h then H_BLOCK (h ' a) else
+              if f a = a then H_EMP else H_REF (f a)`;
+
+val gc_inv_def = Define `
+  gc_inv (h1,roots1,h,f) (b,i,j,e,b2,e2,m,z) =
+    (b <= i /\ i <= j /\ j <= e) /\
+    (* semispaces are disjoint *)
+    (~(e < b2) ==> e2 < b) /\
+    (* EMP outside of b2-e2 and b-j *)
+    (!k. ~(RANGE(b2,e2)k) /\ ~(RANGE(b,j)k) ==> (m k = H_EMP)) /\
+    (* heap full of BLOCK elements between b-i, i-j *)
+    full_heap b i m /\ full_heap i j m /\ 
+    (* data elements from b2-e2 fit into j-e *)
+    (?len. part_heap b2 e2 m len /\ len <= e-j) /\
+    (* refinement *)
+    ref_mem (h,f) m /\ 
+    (* simulation *)
+    ok_heap (h1,roots1) /\ 
+    abs_steps (h1,{},{},ADDR_SET roots1,I) (h,D0(CUT(b,i)m),D0(CUT(i,j)m),z,f)`;
+ 
+(* some lemmas *)
+
+val RANGE_TAC = FULL_SIMP_TAC std_ss [RANGE_def,IN_DEF,gc_inv_def] \\ DECIDE_TAC
+
+val gc_inv_IMP = store_thm("gc_inv_IMP",
+  ``gc_inv (h1,roots1,h,f) (b,i,j,e,b2,e2,m,z) ==>
+    abs_gc_inv (h1,roots1) (h,D0(CUT(b,i)m),D0(CUT(i,j)m),z,f)``,
+  SIMP_TAC std_ss [gc_inv_def] \\ METIS_TAC [ok_heap_IMP,abs_steps_thm]);
+
+val gc_inv_THM = store_thm("gc_inv_THM",
+  ``gc_inv (h1,roots1,h,f) (b,i,j,e,b2,e2,m,z) =
+    gc_inv (h1,roots1,h,f) (b,i,j,e,b2,e2,m,z) /\
+    abs_gc_inv (h1,roots1) (h,D0(CUT(b,i)m),D0(CUT(i,j)m),z,f)``,
+  METIS_TAC [gc_inv_IMP]);
+
+val full_heap_REFL = store_thm("full_heap_REFL",
+  ``!b m. full_heap b b m``, 
+  METIS_TAC [full_heap_cases]);
+
+val full_heap_TRANS = store_thm("full_heap_TRANS",
+  ``!j b i m. full_heap b i m /\ full_heap i j m ==> full_heap b j m``,
+  STRIP_TAC \\ SIMP_TAC std_ss [GSYM AND_IMP_INTRO] \\ HO_MATCH_MP_TAC full_heap_ind
+  \\ ASM_SIMP_TAC std_ss [] \\ REPEAT STRIP_TAC \\ METIS_TAC [full_heap_cases]);
+
+val full_heap_step = prove(
+  ``!n xs d b e m. full_heap b e m ==>
+            (m e = H_BLOCK (xs,n,d)) /\ EMP_RANGE (e+1,e+n+1) m ==>
+            full_heap b (e+n+1) m``,
+  NTAC 3 STRIP_TAC
+  \\ HO_MATCH_MP_TAC full_heap_ind \\ STRIP_TAC THEN1 METIS_TAC [full_heap_cases]
+  \\ REPEAT STRIP_TAC \\ RES_TAC \\ METIS_TAC [full_heap_cases]);
+
+val CUT_EQ = store_thm("CUT_EQ",
+  ``((CUT (b,e) m a = H_BLOCK x) = (a IN RANGE (b,e) /\ (m a = H_BLOCK x))) /\
+    ((CUT (b,e) m a = H_REF i) = (a IN RANGE (b,e) /\ (m a = H_REF i)))``,
+  SIMP_TAC std_ss [CUT_def,IN_DEF] \\ SRW_TAC [] []);
+
+val CUT_update = prove(
+  ``~RANGE (i,j) k ==> (CUT (i,j) ((k =+ x) m) = CUT (i,j) m)``,
+  SIMP_TAC std_ss [CUT_def,UPDATE_def,FUN_EQ_THM] \\ METIS_TAC []);
+
+val part_heap_LESS_EQ = store_thm("part_heap_LESS_EQ",
+  ``!b e m k. part_heap b e m k ==> b <= e``,
+  HO_MATCH_MP_TAC part_heap_ind \\ REPEAT STRIP_TAC \\ DECIDE_TAC);
+
+val EMP_RANGE_RANGE = prove(
+  ``!b e i m.
+      ~(RANGE(b,e)i) ==> (EMP_RANGE (b,e) ((i=+x)m) = EMP_RANGE (b,e) m)``,
+  FULL_SIMP_TAC std_ss [EMP_RANGE_def,APPLY_UPDATE_THM,IN_DEF] \\ METIS_TAC []);
+
+val part_heap_TRANS = store_thm("part_heap_TRANS",
+  ``!j k2 b i m k1. part_heap b i m k1 /\ part_heap i j m k2 ==> part_heap b j m (k1+k2)``,
+  NTAC 2 STRIP_TAC \\ SIMP_TAC std_ss [GSYM AND_IMP_INTRO] 
+  \\ HO_MATCH_MP_TAC part_heap_ind \\ ASM_SIMP_TAC std_ss [] \\ STRIP_TAC
+  THEN1 (REPEAT STRIP_TAC \\ RES_TAC \\ METIS_TAC [part_heap_cases])
+  \\ REPEAT STRIP_TAC \\ RES_TAC \\ ONCE_REWRITE_TAC [part_heap_cases]
+  \\ ASM_SIMP_TAC std_ss [heap_element_11] \\ DISJ2_TAC
+  \\ Q.EXISTS_TAC `k1+k2` \\ ASM_SIMP_TAC std_ss [] \\ DECIDE_TAC);
+
+val part_heap_IGNORE = store_thm("part_heap_IGNORE",
+  ``!b e m k. part_heap b e m k /\ ~(RANGE(b,e)i) ==> 
+              part_heap b e ((i =+ x) m) k``,
+  SIMP_TAC std_ss [GSYM AND_IMP_INTRO] \\ HO_MATCH_MP_TAC part_heap_ind
+  \\ STRIP_TAC THEN1 METIS_TAC [part_heap_cases]
+  \\ STRIP_TAC THEN1
+   (REPEAT STRIP_TAC \\ IMP_RES_TAC part_heap_LESS_EQ
+    \\ `~(RANGE(b+1,e)i) /\ ~(i = b)` by RANGE_TAC \\ RES_TAC
+    \\ METIS_TAC [APPLY_UPDATE_THM,part_heap_cases])
+  \\ REPEAT STRIP_TAC \\ IMP_RES_TAC part_heap_LESS_EQ  
+  \\ `~RANGE (b + n + 1,e) i /\ ~(b = i) /\ ~(RANGE(b+1,b+n+1)i)` by RANGE_TAC
+  \\ ONCE_REWRITE_TAC [part_heap_cases] \\ DISJ2_TAC \\ DISJ2_TAC
+  \\ FULL_SIMP_TAC std_ss [APPLY_UPDATE_THM,heap_element_11,EMP_RANGE_RANGE]);
+  
+val part_heap_EMP_RANGE = store_thm("part_heap_EMP_RANGE",
+  ``!i m. b <= i /\ EMP_RANGE (b,i) m ==> part_heap b i m 0``, 
+  STRIP_TAC \\ completeInduct_on `i-b` \\ REPEAT STRIP_TAC \\ Cases_on `i = b`
+  \\ FULL_SIMP_TAC std_ss [] THEN1 METIS_TAC [part_heap_cases]
+  \\ `b+1 <= i /\ i - (b + 1) < i - b /\ (i - (b + 1) = i - (b + 1))` by DECIDE_TAC
+  \\ ONCE_REWRITE_TAC [part_heap_cases] \\ DISJ2_TAC \\ DISJ1_TAC
+  \\ SUBGOAL `(m b = H_EMP) /\ EMP_RANGE (b+1,i) m` 
+  THEN1 (RES_TAC \\ FULL_SIMP_TAC std_ss [isBLOCK_def,heap_element_distinct])
+  \\ FULL_SIMP_TAC std_ss [EMP_RANGE_def,IN_DEF]
+  \\ `RANGE(b,i)b` by RANGE_TAC \\ ASM_SIMP_TAC std_ss []
+  \\ REPEAT STRIP_TAC \\ `RANGE(b,i)k` by RANGE_TAC \\ ASM_SIMP_TAC std_ss []);
+
+val part_heap_REF = store_thm("part_heap_REF",
+  ``!b e m k. part_heap b e m k /\ (m i = H_BLOCK (x,y,d)) /\ RANGE(b,e)i ==>
+              y+1 <= k /\ part_heap b e ((i =+ H_REF t) m) (k - (y + 1))``,
+  SIMP_TAC std_ss [GSYM AND_IMP_INTRO] \\ HO_MATCH_MP_TAC part_heap_ind
+  \\ STRIP_TAC THEN1 (REPEAT STRIP_TAC \\ `F` by RANGE_TAC)
+  \\ STRIP_TAC THEN1
+   (NTAC 7 STRIP_TAC \\ FULL_SIMP_TAC std_ss [] \\ Cases_on `i = b`
+    THEN1 FULL_SIMP_TAC std_ss [isBLOCK_def,heap_element_11]
+    \\ `RANGE (b + 1,e) i` by RANGE_TAC
+    \\ METIS_TAC [APPLY_UPDATE_THM,part_heap_cases])
+  \\ NTAC 10 STRIP_TAC \\ RES_TAC
+  \\ Cases_on `RANGE (b + n + 1,e) i` THEN1 
+   (`~(i = b)` by RANGE_TAC \\ RES_TAC \\ STRIP_TAC THEN1 DECIDE_TAC
+    \\ ONCE_REWRITE_TAC [part_heap_cases] \\ DISJ2_TAC \\ DISJ2_TAC
+    \\ ASM_SIMP_TAC std_ss [APPLY_UPDATE_THM,heap_element_11]
+    \\ FULL_SIMP_TAC std_ss [EMP_RANGE_def,IN_DEF,APPLY_UPDATE_THM]
+    \\ Q.EXISTS_TAC `k-(y+1)` \\ STRIP_TAC THEN1 RANGE_TAC
+    \\ ASM_SIMP_TAC std_ss [] \\ ALPHA_TAC "j" \\ REPEAT STRIP_TAC
+    \\ Cases_on `i = j` \\ FULL_SIMP_TAC std_ss [heap_element_distinct] \\ RANGE_TAC)
+  \\ Cases_on `RANGE (b + 1,b + n + 1) i` THEN1
+   (FULL_SIMP_TAC std_ss [EMP_RANGE_def,IN_DEF] \\ RES_TAC
+    \\ FULL_SIMP_TAC std_ss [heap_element_distinct])
+  \\ `i = b` by RANGE_TAC \\ FULL_SIMP_TAC std_ss [heap_element_11]
+  \\ ONCE_REWRITE_TAC [part_heap_cases] \\ DISJ2_TAC \\ DISJ1_TAC
+  \\ SIMP_TAC std_ss [isBLOCK_def,APPLY_UPDATE_THM,heap_element_distinct] 
+  \\ FULL_SIMP_TAC std_ss [DECIDE ``k+n+1-(n+1)=k``]
+  \\ MATCH_MP_TAC part_heap_IGNORE \\ REVERSE STRIP_TAC THEN1 RANGE_TAC
+  \\ ONCE_REWRITE_TAC [GSYM (RW1[ADD_COMM]ADD_0)]
+  \\ MATCH_MP_TAC part_heap_TRANS \\ Q.EXISTS_TAC `b+n+1` \\ ASM_SIMP_TAC std_ss []
+  \\ ASM_SIMP_TAC std_ss [part_heap_EMP_RANGE]);
+
+val part_heap_LENGTH_LESS_EQ = store_thm("part_heap_LENGTH_LESS_EQ",
+  ``!b e m k. part_heap b e m k ==> k <= e - b``,
+  HO_MATCH_MP_TAC part_heap_ind \\ ASM_SIMP_TAC std_ss []
+  \\ REPEAT STRIP_TAC \\ IMP_RES_TAC part_heap_LESS_EQ \\ DECIDE_TAC);
+
+val CUT_UPDATE = store_thm("CUT_UPDATE",
+  ``!b e a m x.
+      (~(RANGE(b,e)a) ==> (CUT(b,e)((a=+x)m) = CUT(b,e)m)) /\
+      (RANGE(b,e)a ==> (CUT(b,e)((a=+x)m) = (a=+x)(CUT(b,e)m)))``,
+  FULL_SIMP_TAC std_ss [FUN_EQ_THM,CUT_def,APPLY_UPDATE_THM] \\ METIS_TAC []);
+
+val ref_mem_IMP = prove(
+  ``(ref_mem (h,f) m /\ (m n = H_BLOCK x) ==> n IN FDOM h /\ (h ' n = x)) /\
+    (ref_mem (h,f) m /\ (m n = H_REF i) ==> ~(n IN FDOM h) /\ ~(f n = n) /\ (f n = i)) /\
+    (ref_mem (h,f) m /\ (m n = H_EMP) ==> ~(n IN FDOM h) /\ (f n = n))``,
+  SIMP_TAC std_ss [ref_mem_def,GSYM AND_IMP_INTRO] 
+  \\ METIS_TAC [heap_element_11,heap_element_distinct]);
+
+val full_heap_LESS_EQ = store_thm("full_heap_LESS_EQ",
+  ``!b e m. full_heap b e m ==> b <= e``,
+  HO_MATCH_MP_TAC full_heap_ind \\ REPEAT STRIP_TAC \\ DECIDE_TAC);
+
+val full_heap_RANGE = store_thm("full_heap_RANGE",
+  ``!i x b e m. full_heap b e m /\ ~(RANGE(b,e)i) ==> full_heap b e ((i =+ x) m)``,
+  NTAC 2 STRIP_TAC \\ SIMP_TAC std_ss [GSYM AND_IMP_INTRO]
+  \\ HO_MATCH_MP_TAC full_heap_ind \\ REPEAT STRIP_TAC
+  \\ ONCE_REWRITE_TAC [full_heap_cases] \\ SIMP_TAC std_ss [APPLY_UPDATE_THM]
+  \\ IMP_RES_TAC full_heap_LESS_EQ
+  \\ `~RANGE (b + n + 1,e) i /\ ~(b = i) /\ ~(RANGE(b+1,b+n+1)i)` by
+       (FULL_SIMP_TAC std_ss [RANGE_def] \\ DECIDE_TAC)
+  \\ FULL_SIMP_TAC std_ss [heap_element_11,EMP_RANGE_RANGE]);
+
+val full_heap_R0 = prove(
+  ``!b e m. full_heap b e m ==> !k. RANGE(b,e)k ==> ~(R0 m k)``,
+  HO_MATCH_MP_TAC full_heap_ind \\ REPEAT STRIP_TAC 
+  THEN1 (FULL_SIMP_TAC std_ss [RANGE_def] \\ DECIDE_TAC)
+  \\ Cases_on `b = k` \\ FULL_SIMP_TAC std_ss [R0,heap_element_distinct]
+  \\ FULL_SIMP_TAC std_ss [EMP_RANGE_def,IN_DEF,heap_element_distinct]
+  \\ Cases_on `RANGE (b + n + 1,e) k` THEN1 METIS_TAC []
+  \\ `RANGE (b + 1,b + n + 1) k` by (FULL_SIMP_TAC std_ss [RANGE_def] \\ DECIDE_TAC)
+  \\ RES_TAC \\ FULL_SIMP_TAC std_ss [R0,heap_element_distinct]);
+
+(* proof *)
+
+val move_lemma = store_thm("move_lemma",
+  ``gc_inv (h1,roots1,h,f) (b,i,j,e,b2,e2,m,z UNION {n}) /\
+    n IN (DR0(CUT(b2,e2)m)) ==>
+    (m n = H_REF (f n)) /\ ~(f n = n) \/
+    getLENGTH (m n) <= e - j /\ (m n = H_BLOCK (h ' n)) /\ n IN FDOM h /\ ~(n = j) /\
+    n IN RANGE(b2,e2) /\ (f n = n) /\ EMP_RANGE (j,j+getLENGTH(H_BLOCK (h ' n))) m``,
+  PURE_ONCE_REWRITE_TAC [gc_inv_THM] \\ ONCE_REWRITE_TAC [IN_DEF] \\ STRIP_TAC
+  \\ FULL_SIMP_TAC std_ss [gc_inv_def] \\ FULL_SIMP_TAC std_ss [DR0,R0,D0,CUT_EQ]
+  \\ IMP_RES_TAC ref_mem_IMP \\ ASM_SIMP_TAC std_ss [heap_element_11,heap_element_distinct]
+  \\ SIMP_TAC std_ss [getLENGTH_def] \\ `n < e2` by RANGE_TAC
+  \\ `(CUT(b2,e2)m) n = H_BLOCK (x,y,z')` by FULL_SIMP_TAC std_ss [CUT_EQ]
+  \\ FULL_SIMP_TAC std_ss [IN_DEF]
+  \\ IMP_RES_TAC part_heap_REF \\ STRIP_TAC THEN1 RANGE_TAC
+  \\ FULL_SIMP_TAC std_ss [abs_gc_inv_def,LET_DEF]
+  \\ STRIP_TAC THEN1 RANGE_TAC
+  \\ STRIP_TAC THEN1
+      (`n IN FDOM h` by FULL_SIMP_TAC std_ss [IN_DEF] \\ CCONTR_TAC
+       \\ `n IN D0 (CUT (i,j) m) \/ n IN D0 (CUT (b,i) m)` by METIS_TAC []
+       \\ FULL_SIMP_TAC std_ss [D0,CUT_EQ,IN_DEF] \\ RANGE_TAC)
+   \\ FULL_SIMP_TAC std_ss [EMP_RANGE_def,IN_DEF]
+   \\ REPEAT STRIP_TAC \\ Q.PAT_ASSUM `!k. bbb ==> (m k = H_EMP)` MATCH_MP_TAC 
+   \\ RANGE_TAC);
+
+val ADDR_SET_THM = store_thm("ADDR_SET_THM",
+  ``(ADDR_SET [] = {}) /\
+    (ADDR_SET (H_DATA x :: xs) = ADDR_SET xs) /\
+    (ADDR_SET (H_ADDR y :: xs) = y INSERT ADDR_SET xs)``,
+  SRW_TAC [] [ADDR_SET_def,EXTENSION,MEM,NOT_IN_EMPTY,IN_INSERT]);
+
+val CUT_EMPTY = store_thm("CUT_EMPTY",
+  ``(D0(CUT(j,j)m) = {}) /\ (D1(CUT(j,j)m) = {}) /\
+    (R0(CUT(j,j)m) = {}) /\ (R1(CUT(j,j)m) = {})``,
+  SIMP_TAC std_ss [EXTENSION,NOT_IN_EMPTY]
+  \\ `!j n. ~RANGE(j,j)n` by RANGE_TAC
+  \\ ASM_SIMP_TAC std_ss [IN_DEF,D0,R0,D1,R1,CUT_EQ]);
+
+val remove_from_z = prove(
+  ``~(f n = n) ==> abs_steps (h,x,y,z UNION {n},f) (h,x,y,z,f)``,
+  REPEAT STRIP_TAC \\ SIMP_TAC std_ss [abs_steps_def] \\ Cases_on `n IN z`
+  THEN1 (`z UNION {n} = z` by SET_TAC \\ FULL_SIMP_TAC std_ss [RTC_REFL])
+  \\ `(z,f) = ((z UNION {n}) DELETE n,f)` by SET_TAC
+  \\ POP_ASSUM (fn th => ONCE_REWRITE_TAC [th]) \\ MATCH_MP_TAC RTC_SINGLE
+  \\ SIMP_TAC std_ss [abs_step_cases] \\ SET_TAC);  
+
+val full_heap_BLOCK = prove(
+  ``!b e m. full_heap b e m /\ (m i = H_BLOCK (x2,y,z2)) ==> 
+            full_heap b e ((i =+ H_BLOCK (x,y,z)) m)``,
+  SIMP_TAC std_ss [GSYM AND_IMP_INTRO] \\ HO_MATCH_MP_TAC full_heap_ind
+  \\ SIMP_TAC std_ss [full_heap_REFL] \\ REPEAT STRIP_TAC \\ RES_TAC
+  \\ ONCE_REWRITE_TAC [full_heap_cases] 
+  \\ FULL_SIMP_TAC std_ss [EMP_RANGE_def,IN_DEF,APPLY_UPDATE_THM]
+  \\ METIS_TAC [heap_element_11,heap_element_distinct,PAIR_EQ]);
+
+val move_thm = store_thm("move_thm",
+  ``gc_inv (h1,roots1,h,f) (b,i,j,e,b2,e2,m,z UNION ADDR_SET [x]) /\
+    ADDR_SET [x] SUBSET (DR0(CUT(b2,e2)m)) /\
+    (move (x,j,m) = (x2,j2,m2)) ==>
+      ?h2 f2. gc_inv (h1,roots1,h2,f2) (b,i,j2,e,b2,e2,m2,z UNION (D1(CUT(j,j2)m2))) /\ j <= j2 /\
+              DR0 (CUT (b2,e2) m) SUBSET DR0 (CUT (b2,e2) m2) /\
+              (CUT(b,j)m = CUT(b,j)m2) /\
+              (!a. ~(f a = a) ==> (f2 a = f a)) /\
+              (!a. a IN ADDR_SET [x2] ==> ~(f2 a = a)) /\
+              ([x2] = ADDR_MAP f2 [x]) /\ full_heap j j2 m2``,
+  CONV_TAC (RATOR_CONV (ONCE_REWRITE_CONV [gc_inv_THM]))
+  \\ REVERSE (Cases_on `x`) THEN1
+   (SIMP_TAC std_ss [move_def] \\ ONCE_REWRITE_TAC [EQ_SYM_EQ]
+    \\ `ADDR_SET [H_DATA a] = {}` by ALL_TAC \\ ASM_SIMP_TAC std_ss [full_heap_REFL]
+    \\ ASM_SIMP_TAC std_ss [ADDR_SET_def,SUBSET_DEF,MEM,NOT_IN_EMPTY,ADDR_MAP_def,
+          heap_address_distinct,EXTENSION,UNION_EMPTY,CUT_EMPTY] \\ SET_TAC)
+  \\ SIMP_TAC std_ss [ADDR_SET_THM,INSERT_SUBSET,EMPTY_SUBSET]
+  \\ STRIP_TAC
+  \\ IMP_RES_TAC move_lemma \\ FULL_SIMP_TAC std_ss [heap_element_distinct]
+  THEN1
+   (Q.LIST_EXISTS_TAC [`h`,`f`] \\ ASM_SIMP_TAC std_ss []
+    \\ Q.PAT_ASSUM `move xx = fg` MP_TAC \\ ASM_SIMP_TAC (srw_ss()) [move_def]
+    \\ ONCE_REWRITE_TAC [EQ_SYM_EQ] \\ SIMP_TAC std_ss [ADDR_SET_THM,
+         IN_INSERT,NOT_IN_EMPTY,CUT_EMPTY,UNION_EMPTY,full_heap_REFL] 
+    \\ FULL_SIMP_TAC std_ss [gc_inv_def,ADDR_MAP_def] \\ IMP_RES_TAC remove_from_z 
+    \\ `f o f = I` by METIS_TAC [abs_gc_inv_def] \\ FULL_SIMP_TAC std_ss [FUN_EQ_THM]
+    \\ METIS_TAC [abs_steps_thm,remove_from_z,abs_steps_TRANS])
+  \\ `?x y d. h ' n = (x,y,d)` by METIS_TAC [PAIR]
+  \\ Q.PAT_ASSUM `move xx = fg` MP_TAC \\ ASM_SIMP_TAC (srw_ss()) [move_def]
+  \\ ONCE_REWRITE_TAC [EQ_SYM_EQ] \\ SIMP_TAC std_ss [LET_DEF,DECIDE ``j <= j + y + 1``]  
+  \\ STRIP_TAC 
+  \\ Q.LIST_EXISTS_TAC [`h |+ (j,h ' n) \\ n`,`(n =+ j) ((j =+ n) f)`] \\ ASM_SIMP_TAC std_ss []
+  \\ FULL_SIMP_TAC std_ss [APPLY_UPDATE_THM,ADDR_SET_THM,IN_INSERT,NOT_IN_EMPTY]
+  \\ `full_heap j (j + y + 1) ((j =+ H_BLOCK (x,y,d)) ((n =+ H_REF j) m))` by ALL_TAC THEN1
+    (Q.PAT_ASSUM `~(n = j)` (fn th => REWRITE_TAC [MATCH_MP UPDATE_COMMUTES (GSYM th)])
+     \\ `~(RANGE(j,j+y+1)n)` by ALL_TAC THEN1
+      (REPEAT STRIP_TAC \\ FULL_SIMP_TAC std_ss [IN_DEF,R0,D0,DR0,EMP_RANGE_def,
+         getLENGTH_def,ADD_ASSOC,heap_element_distinct])
+     \\ MATCH_MP_TAC full_heap_RANGE \\ ASM_SIMP_TAC std_ss []
+     \\ ONCE_REWRITE_TAC [full_heap_cases] \\ DISJ2_TAC
+     \\ FULL_SIMP_TAC std_ss [APPLY_UPDATE_THM,heap_element_11,full_heap_REFL,
+          EMP_RANGE_def,getLENGTH_def,IN_DEF,ADD_ASSOC] \\ REPEAT STRIP_TAC 
+     \\ `~(j = k) /\ RANGE (j,j + y + 1) k` by RANGE_TAC \\ SET_TAC)
+  \\ REVERSE STRIP_TAC THEN1
+   (`~(RANGE(b,j)j) /\ ~(RANGE(b,j)n) /\ ~(RANGE(b2,e2)j)` by RANGE_TAC
+    \\ ASM_SIMP_TAC std_ss [CUT_UPDATE,ADDR_MAP_def] 
+    \\ FULL_SIMP_TAC std_ss [SUBSET_DEF,DR0,IN_DEF,D0,R0,CUT_EQ,APPLY_UPDATE_THM]   
+    \\ FULL_SIMP_TAC std_ss [getLENGTH_def,EMP_RANGE_def,ADD_ASSOC,IN_DEF]  
+    \\ `RANGE (j,j + y + 1) j` by RANGE_TAC
+    \\ FULL_SIMP_TAC std_ss [gc_inv_def,FUN_EQ_THM,abs_gc_inv_def,LET_DEF]
+    \\ `f j = j` by METIS_TAC [ref_mem_def,heap_element_distinct]
+    \\ REPEAT STRIP_TAC \\ METIS_TAC [heap_element_11,heap_element_distinct,PAIR_EQ])
+  \\ FULL_SIMP_TAC std_ss [gc_inv_def]
+  \\ FULL_SIMP_TAC std_ss [getLENGTH_def]
+  \\ `~(RANGE(b,i)j) /\ ~(RANGE(b,i)n) /\ ~(RANGE(i,j)j) /\ 
+      ~(RANGE(i,j)n) /\ ~(RANGE(b2,e2)j)` by RANGE_TAC
+  \\ REPEAT STRIP_TAC THEN1 RANGE_TAC THEN1 RANGE_TAC
+  THEN1 (`~(j = k) /\ ~(n = k) /\ ~RANGE (b,j) k` by RANGE_TAC \\ METIS_TAC [APPLY_UPDATE_THM])
+  THEN1 METIS_TAC [full_heap_RANGE]
+  THEN1
+   (MATCH_MP_TAC full_heap_TRANS \\ Q.EXISTS_TAC `j` \\ ASM_SIMP_TAC std_ss [full_heap_RANGE])
+  THEN1  
+   (Q.EXISTS_TAC `len - (y+1)` \\ FULL_SIMP_TAC std_ss [IN_DEF]
+    \\ IMP_RES_TAC (Q.INST [`t`|->`j`] part_heap_REF)
+    \\ REVERSE STRIP_TAC THEN1 DECIDE_TAC    
+    \\ MATCH_MP_TAC part_heap_IGNORE \\ ASM_SIMP_TAC std_ss [])
+  THEN1
+   (SIMP_TAC std_ss [ref_mem_def,APPLY_UPDATE_THM,FDOM_FUPDATE,FDOM_DOMSUB,
+      IN_INSERT,IN_DELETE,FAPPLY_FUPDATE_THM,DOMSUB_FAPPLY_THM] 
+    \\ ALPHA_TAC "k" \\ REPEAT STRIP_TAC 
+    \\ Cases_on `j = k` \\ FULL_SIMP_TAC std_ss []
+    \\ Cases_on `k = n` \\ FULL_SIMP_TAC std_ss [ref_mem_def])
+  \\ FULL_SIMP_TAC std_ss [CUT_UPDATE]
+  \\ Q.PAT_ASSUM `~(n = j)` (fn th => REWRITE_TAC [MATCH_MP UPDATE_COMMUTES (GSYM th)] THEN ASSUME_TAC th)
+  \\ `~(RANGE(j,j + y + 1)n) /\ ~(RANGE(i,j + y + 1)n)` by RANGE_TAC
+  \\ FULL_SIMP_TAC std_ss [CUT_UPDATE]
+  \\ REPEAT (Q.PAT_ASSUM `~(RANGE(xx,yy)df)` (K ALL_TAC))
+  \\ `!k. RANGE (i,j + y + 1) k /\ ~RANGE (i,j) k  ==> RANGE (j,j + y + 1) k` by RANGE_TAC
+  \\ `D0 (CUT (i,j + y + 1) ((j =+ H_BLOCK (x,y,d)) m)) =
+       j INSERT D0 (CUT (i,j) m)` by ALL_TAC THEN1
+     (FULL_SIMP_TAC std_ss [EXTENSION,IN_INSERT] 
+      \\ FULL_SIMP_TAC std_ss [IN_DEF,D0,CUT_EQ,APPLY_UPDATE_THM,EMP_RANGE_def,IN_DEF]
+      \\ REPEAT STRIP_TAC \\ EQ_TAC \\ REPEAT STRIP_TAC THEN1
+       (Cases_on `j = x'` \\ FULL_SIMP_TAC std_ss [heap_element_11] 
+        \\ CCONTR_TAC \\ `RANGE(j,j+y+1)x'` by RANGE_TAC 
+        \\ METIS_TAC [heap_element_distinct,ADD_ASSOC])
+      \\ Cases_on `j = x'` \\ FULL_SIMP_TAC std_ss [heap_element_11] \\ RANGE_TAC)  
+  \\ `D1 (CUT (j,j + y + 1) ((j =+ H_BLOCK (x,y,d)) m)) = ADDR_SET x` by 
+     (FULL_SIMP_TAC std_ss [FUN_EQ_THM,D1,CUT_EQ,IN_DEF,APPLY_UPDATE_THM,EMP_RANGE_def] 
+      \\ REPEAT STRIP_TAC \\ EQ_TAC \\ REPEAT STRIP_TAC 
+      THEN1 (Cases_on `j = k` \\ METIS_TAC 
+        [heap_element_11,heap_element_distinct,PAIR_EQ,ADD_ASSOC])
+      \\ Q.EXISTS_TAC `j` \\ ASM_SIMP_TAC std_ss [heap_element_11] \\ RANGE_TAC)
+  \\ ASM_SIMP_TAC std_ss []
+  \\ MATCH_MP_TAC abs_steps_TRANS
+  \\ Q.EXISTS_TAC `(h,D0 (CUT (b,i) m),D0 (CUT (i,j) m),z UNION {n},f)`
+  \\ ASM_SIMP_TAC std_ss []
+  \\ MATCH_MP_TAC abs_steps_TRANS
+  \\ Q.EXISTS_TAC `(h |+ (j,x,y,d) \\ n,D0 (CUT (b,i) m),j INSERT D0 (CUT (i,j) m),
+       (z UNION ADDR_SET x) UNION {n},(n =+ j) ((j =+ n) f))`
+  \\ REVERSE STRIP_TAC
+  THEN1 (MATCH_MP_TAC remove_from_z \\ ASM_SIMP_TAC std_ss [APPLY_UPDATE_THM])
+  \\ `!xx. z UNION xx UNION {n} = z UNION {n} UNION xx` by SET_TAC
+  \\ ASM_SIMP_TAC std_ss []
+  \\ SIMP_TAC std_ss [abs_steps_def] \\ MATCH_MP_TAC RTC_SINGLE
+  \\ SIMP_TAC std_ss [abs_step_cases] \\ DISJ2_TAC \\ DISJ2_TAC
+  \\ Q.LIST_EXISTS_TAC [`n`,`j`,`x`,`(y,d)`] \\ ASM_SIMP_TAC std_ss []
+  \\ STRIP_TAC THEN1 SET_TAC    
+  \\ `~RANGE (b2,e2) j /\ ~RANGE (b,j) j` by RANGE_TAC 
+  \\ `m j = H_EMP` by SET_TAC 
+  \\ Q.PAT_ASSUM `ref_mem (h,f) m` (fn th => FULL_SIMP_TAC std_ss [RW[ref_mem_def]th])
+  \\ METIS_TAC [heap_element_distinct,IN_UNION,IN_INSERT]);
+
+val ADDR_SET_CONS = store_thm("ADDR_SET_CONS",
+  ``!h xs. ADDR_SET (h::xs) = ADDR_SET xs UNION ADDR_SET [h]``,
+  Cases \\ FULL_SIMP_TAC std_ss [ADDR_SET_THM,EXTENSION,IN_UNION] \\ SET_TAC);
+
+val D1_UNION = store_thm("D1_UNION",
+  ``b <= i /\ i <= j ==> (D1(CUT(b,j)m) = D1(CUT(b,i)m) UNION D1(CUT(i,j)m)) /\
+                         (D0(CUT(b,j)m) = D0(CUT(b,i)m) UNION D0(CUT(i,j)m))``,
+  SIMP_TAC std_ss [EXTENSION,IN_UNION] \\ SIMP_TAC std_ss [IN_DEF,D1,CUT_EQ,D0]
+  \\ REPEAT STRIP_TAC \\ `!k. RANGE(b,j)k = RANGE(b,i)k \/ RANGE(i,j)k` by RANGE_TAC
+  \\ SET_TAC);
+
+val D1_CUT_EQ_ADDR_SET_THM = prove(
+  ``(m j = H_BLOCK (x,y,d)) /\ EMP_RANGE (j+1,j+y+1) m ==>
+    (D1 (CUT (j,j + y + 1) m) = ADDR_SET x)``,
+  FULL_SIMP_TAC std_ss [FUN_EQ_THM,D1,CUT_EQ,IN_DEF,APPLY_UPDATE_THM,EMP_RANGE_def] 
+  \\ REPEAT STRIP_TAC \\ EQ_TAC \\ REPEAT STRIP_TAC 
+  THEN1 (Cases_on `j = k` \\ FULL_SIMP_TAC std_ss [EMP_RANGE_def,IN_DEF]
+         THEN1 METIS_TAC [heap_element_11,heap_element_distinct,PAIR_EQ,ADD_ASSOC]
+         \\ `RANGE (j + 1,j + y + 1) k` by RANGE_TAC 
+         \\ METIS_TAC [heap_element_distinct])
+  \\ Q.EXISTS_TAC `j` \\ ASM_SIMP_TAC std_ss [heap_element_11] \\ RANGE_TAC);
+
+val EQ_RANGE_def = Define `
+  EQ_RANGE (b,e) m m2 = !k. k IN RANGE (b,e) ==> (m k = m2 k)`;
+
+val EQ_RANGE_IMP_EQ_RANGE = store_thm("EQ_RANGE_IMP_EQ_RANGE",
+  ``!b e i j m m2. EQ_RANGE (b,e) m m2 /\ b <= i /\ j <= e ==> EQ_RANGE (i,j) m m2``,
+  SIMP_TAC std_ss [EQ_RANGE_def,IN_DEF,RANGE_def] \\ REPEAT STRIP_TAC
+  \\ Q.PAT_ASSUM `!k.bbb` MATCH_MP_TAC \\ DECIDE_TAC);
+
+val EQ_RANGE_full_heap = store_thm("EQ_RANGE_full_heap",
+  ``!m2 b e m. full_heap b e m /\ EQ_RANGE (b,e) m m2 ==> full_heap b e m2``,
+  STRIP_TAC \\ SIMP_TAC std_ss [GSYM AND_IMP_INTRO] \\ HO_MATCH_MP_TAC full_heap_ind
+  \\ REPEAT STRIP_TAC THEN1 METIS_TAC [full_heap_cases]
+  \\ ONCE_REWRITE_TAC [full_heap_cases] \\ IMP_RES_TAC full_heap_LESS_EQ
+  \\ `~(e = b)` by DECIDE_TAC \\ ASM_SIMP_TAC std_ss []
+  \\ `b IN RANGE (b,e)` by (SIMP_TAC std_ss [RANGE_def,IN_DEF] \\ DECIDE_TAC)
+  \\ `m2 b = m b` by METIS_TAC [EQ_RANGE_def] 
+  \\ ASM_SIMP_TAC std_ss [heap_element_11] 
+  \\ `b <= b + n + 1 /\ e <= e` by DECIDE_TAC \\ REVERSE STRIP_TAC
+  THEN1 (IMP_RES_TAC EQ_RANGE_IMP_EQ_RANGE \\ RES_TAC \\ ASM_SIMP_TAC std_ss []) 
+  \\ FULL_SIMP_TAC std_ss [EMP_RANGE_def,IN_DEF]
+  \\ REPEAT STRIP_TAC \\ RES_TAC  
+  \\ REVERSE (`k IN RANGE (b,e)` by ALL_TAC) THEN1 METIS_TAC [EQ_RANGE_def]
+  \\ FULL_SIMP_TAC std_ss [RANGE_def,IN_DEF] \\ DECIDE_TAC);
+
+val EQ_RANGE_CUT = store_thm("EQ_RANGE_CUT",
+  ``EQ_RANGE (b,i) m (CUT (b,i) m)``,
+  SIMP_TAC std_ss [EQ_RANGE_def,CUT_def,IN_DEF]);
+
+val EQ_RANGE_THM = store_thm("EQ_RANGE_THM",
+  ``(CUT (b,e) m1 = CUT (b,e) m2) ==> EQ_RANGE (b,e) m1 m2``,
+  FULL_SIMP_TAC std_ss [CUT_def,FUN_EQ_THM,EQ_RANGE_def,IN_DEF] \\ SET_TAC);
+
+val move_list_thm = store_thm("move_list_thm",
+  ``!xs z h f m j xs2 j2 (m2:num -> ('a,'b) heap_element).
+      gc_inv (h1,roots1,h,f) (b,i,j,e,b2,e2,m,z UNION ADDR_SET xs) /\
+      ADDR_SET xs SUBSET (DR0(CUT(b2,e2)m)) /\
+      (move_list (xs,j,m) = (xs2,j2,m2)) ==>
+        ?h3 f3. gc_inv (h1,roots1,h3,f3) (b,i,j2,e,b2,e2,m2,z UNION (D1(CUT(j,j2)m2))) /\ j <= j2 /\
+                DR0 (CUT (b2,e2) m) SUBSET DR0 (CUT (b2,e2) m2) /\
+                (CUT(b,j)m = CUT(b,j)m2) /\
+                (!a. ~(f a = a) ==> (f3 a = f a)) /\
+                (!a. a IN ADDR_SET xs2 ==> ~(f3 a = a)) /\
+                (xs2 = ADDR_MAP f3 xs) /\ full_heap j j2 m2``,
+  Induct \\ SIMP_TAC std_ss [ADDR_SET_THM,UNION_EMPTY,move_list_def,ADDR_MAP_def,
+    NOT_IN_EMPTY,CUT_EMPTY,LET_DEF,full_heap_REFL] THEN1 SET_TAC
+  \\ ONCE_REWRITE_TAC [ADDR_SET_CONS]
+  \\ NTAC 6 STRIP_TAC \\ FULL_SIMP_TAC std_ss [UNION_SUBSET]     
+  \\ `?x3 j3 m3. move (h,j,m) = (x3,j3,m3)` by METIS_TAC [PAIR]
+  \\ `?xs4 j4 m4. move_list (xs,j3,m3) = (xs4,j4,m4)` by METIS_TAC [PAIR]
+  \\ FULL_SIMP_TAC std_ss [UNION_ASSOC] \\ ONCE_REWRITE_TAC [EQ_SYM_EQ]
+  \\ REPEAT STRIP_TAC
+  \\ IMP_RES_TAC move_thm \\ Q.PAT_ASSUM `!z roots1 i. bb` (K ALL_TAC)
+  \\ Q.PAT_ASSUM `!z h f.bbb` (MP_TAC o Q.SPECL [
+       `z UNION D1(CUT(j,j3)(m3:num -> ('a,'b) heap_element))`,
+       `h2`,`f2`,`m3`,`j3`,`xs4`,`j4`,`m4`]) 
+  \\ `ADDR_SET xs SUBSET DR0 (CUT (b2,e2) m3)` by SET_TAC
+  \\ FULL_SIMP_TAC std_ss [AC UNION_ASSOC UNION_COMM]
+  \\ REPEAT STRIP_TAC \\ FULL_SIMP_TAC std_ss [IN_UNION]
+  \\ Q.LIST_EXISTS_TAC [`h3`,`f3`] \\ `j <= j4` by DECIDE_TAC
+  \\ ONCE_REWRITE_TAC [ADDR_SET_CONS] \\ ASM_SIMP_TAC std_ss []
+  \\ `(CUT (b,j) m3 = CUT (b,j) m4) /\ (CUT (j,j3) m3 = CUT (j,j3) m4)` by 
+      (`!k. k < j ==> k < j3` by DECIDE_TAC
+       \\ `!k. j <= k ==> b <= k` by RANGE_TAC
+       \\ FULL_SIMP_TAC std_ss [CUT_def,RANGE_def,FUN_EQ_THM] \\ SET_TAC)
+  \\ IMP_RES_TAC EQ_RANGE_THM \\ IMP_RES_TAC EQ_RANGE_full_heap 
+  \\ IMP_RES_TAC full_heap_TRANS \\ ASM_SIMP_TAC std_ss []
+  \\ REVERSE STRIP_TAC THEN1
+   (ASM_SIMP_TAC std_ss [] \\ STRIP_TAC THEN1 SET_TAC \\ STRIP_TAC THEN1 SET_TAC
+    \\ Cases_on `h` \\ FULL_SIMP_TAC std_ss [ADDR_MAP_def,CONS_11,
+      ADDR_SET_def,MEM,heap_address_11] \\ IMP_RES_TAC gc_inv_IMP    
+    \\ `f2 (f2 n) = n` by FULL_SIMP_TAC std_ss [gc_inv_def,FUN_EQ_THM,abs_gc_inv_def,LET_DEF]
+    \\ FULL_SIMP_TAC std_ss [])
+  \\ `D1 (CUT (j,j4) m4) = D1 (CUT (j,j3) m4) UNION D1 (CUT (j3,j4) m4)`
+       by METIS_TAC [D1_UNION] \\ FULL_SIMP_TAC std_ss [AC UNION_ASSOC UNION_COMM]);
+
+val D0_UPDATE = store_thm("D0_UPDATE",
+  ``!i x m. i IN D0 m ==> (D0 ((i =+ H_BLOCK x) m) = D0 m)``,
+  SIMP_TAC std_ss [FORALL_PROD,FUN_EQ_THM,IN_DEF,D0,CUT_EQ,APPLY_UPDATE_THM]
+  \\ METIS_TAC []);
+
+val gc_step_lemma = store_thm("gc_step_lemma",
+  ``gc_inv (h1,roots1,h,f) (b,i,j,e,b2,e2,m,D1(CUT(i,j)m)) ==> ~(i = j) ==>
+    ?xs n d. (m i = H_BLOCK (xs,n,d)) /\
+             EMP_RANGE (i + 1,i + n + 1) m /\
+             full_heap (i + n + 1) j m /\
+             ADDR_SET xs SUBSET DR0 (CUT (b2,e2) m) /\
+             (D1 (CUT (i,j) m) = D1 (CUT (i+n+1,j) m) UNION ADDR_SET xs)``,
+  SIMP_TAC std_ss [gc_step_def,LET_DEF] \\ REPEAT STRIP_TAC \\ IMP_RES_TAC gc_inv_IMP
+  \\ `full_heap i j m` by METIS_TAC [gc_inv_def] \\ POP_ASSUM MP_TAC
+  \\ ONCE_REWRITE_TAC [full_heap_cases] \\ ASM_SIMP_TAC std_ss [] \\ STRIP_TAC
+  \\ ASM_SIMP_TAC std_ss [heap_element_11] \\ STRIP_TAC THEN1 METIS_TAC [full_heap_cases]
+  \\ IMP_RES_TAC full_heap_LESS_EQ 
+  \\ `i < i + n + 1 /\ i <= i + n + 1` by DECIDE_TAC
+  \\ `D1 (CUT (i,j) m) = D1 (CUT (i+n+1,j) m) UNION ADDR_SET xs`
+       by METIS_TAC [D1_UNION,D1_CUT_EQ_ADDR_SET_THM,UNION_COMM] 
+  \\ ASM_SIMP_TAC std_ss []
+  \\ `i IN FDOM h /\ (h ' i = (xs,n,d))` by METIS_TAC [gc_inv_def,
+       ref_mem_def, heap_element_distinct,heap_element_11,PAIR_EQ]
+    \\ `i IN (UNIV DIFF D0 (CUT (b,i) m))` by ALL_TAC THEN1
+      (FULL_SIMP_TAC std_ss [IN_DIFF,IN_UNIV]
+       \\ FULL_SIMP_TAC std_ss [IN_DEF,D0,CUT_EQ,heap_element_11] \\ RANGE_TAC)
+    \\ `ADDR_SET xs SUBSET POINTERS h (U(:num) DIFF D0 (CUT (b,i) m))`
+         by METIS_TAC [set_SUBSET_POINTERS]        
+    \\ `D0 (CUT (b,i) m) UNION D0 (CUT (i,j) m) = D0 (CUT(b,j)m)`
+         by METIS_TAC [D1_UNION,gc_inv_def,abs_gc_inv_def] 
+    \\ `ADDR_SET xs SUBSET (FDOM h UNION HAS_CHANGED f DIFF (D0 (CUT (b,j) m)))` by 
+         (FULL_SIMP_TAC std_ss [gc_inv_def,abs_gc_inv_def,LET_DEF] \\ SET_TAC)
+    \\ SIMP_TAC std_ss [SUBSET_DEF] \\ REPEAT STRIP_TAC
+    \\ `x IN (FDOM h UNION HAS_CHANGED f DIFF D0 (CUT (b,j) m))` by SET_TAC
+    \\ Cases_on `x IN FDOM h` THEN1
+     (`~(x IN D0 (CUT (b,j) m))` by SET_TAC
+      \\ POP_ASSUM MP_TAC \\ SIMP_TAC std_ss [IN_DEF,D0,CUT_EQ]
+      \\ `?x1 y1 d1. h ' x = (x1,y1,d1)` by METIS_TAC [PAIR]
+      \\ `m x = H_BLOCK (x1,y1,d1)` by METIS_TAC [ref_mem_def,gc_inv_def]
+      \\ FULL_SIMP_TAC std_ss [heap_element_11,DR0,D0,R0,CUT_EQ,
+           heap_element_distinct,IN_DEF] \\ CCONTR_TAC
+      \\ FULL_SIMP_TAC std_ss [gc_inv_def,abs_gc_inv_def,LET_DEF] 
+      \\ METIS_TAC [heap_element_distinct])
+    \\ FULL_SIMP_TAC std_ss [IN_DIFF,IN_UNION]
+    \\ Q.PAT_ASSUM `~(x IN D0 (CUT (b,j) m))` MP_TAC
+    \\ SIMP_TAC std_ss [IN_DEF,D0,CUT_EQ]
+    \\ FULL_SIMP_TAC std_ss [HAS_CHANGED_def]
+    \\ FULL_SIMP_TAC std_ss [gc_inv_def,abs_gc_inv_def,LET_DEF] 
+    \\ `m x = H_REF (f x)` by METIS_TAC [ref_mem_def]         
+    \\ FULL_SIMP_TAC std_ss [heap_element_distinct,DR0,D0,R0,CUT_EQ,heap_element_11]
+    \\ SIMP_TAC std_ss [IN_DEF]
+    \\ `full_heap b j m` by METIS_TAC [full_heap_TRANS]   
+    \\ `R0 m x` by FULL_SIMP_TAC std_ss [R0,heap_element_11]
+    \\ CCONTR_TAC \\ METIS_TAC [full_heap_R0,heap_element_distinct]); 
+  
+val gc_step_thm = store_thm("gc_step_thm",
+  ``gc_inv (h1,roots1,h,f) (b,i,j,e,b2,e2,m,D1(CUT(i,j)m)) /\ ~(i = j) ==>
+    (gc_step (i,j,m) = (i2,j2,m2)) ==>
+    ?h3 f3. gc_inv (h1,roots1,h3,f3) (b,i2,j2,e,b2,e2,m2,D1(CUT(i2,j2)m2)) /\ 
+            i < i2 /\ j <= j2 /\ !a. ~(f a = a) ==> (f3 a = f a)``,
+  STRIP_TAC \\ IMP_RES_TAC gc_inv_IMP \\ STRIP_ASSUME_TAC (UNDISCH_ALL gc_step_lemma)
+  \\ ASM_SIMP_TAC std_ss [gc_step_def,LET_DEF,getBLOCK_def] 
+  \\ `?xs3 j3 m3. move_list (xs,j,m) = (xs3,j3,m3)` by METIS_TAC [PAIR]
+  \\ FULL_SIMP_TAC std_ss [] \\ REPEAT STRIP_TAC \\ helperLib.EXPAND_TAC
+  \\ `~RANGE(i + n + 1,j3)i` by RANGE_TAC \\ FULL_SIMP_TAC std_ss [CUT_UPDATE]
+  \\ IMP_RES_TAC full_heap_LESS_EQ 
+  \\ `i < i + n + 1 /\ i <= i + n + 1` by DECIDE_TAC
+  \\ FULL_SIMP_TAC std_ss []
+  \\ Q.PAT_ASSUM `gc_inv (h1,roots1,h,f) xxx` (fn th => ASSUME_TAC th THEN 
+       MP_TAC (Q.INST [`xs2`|->`xs3`,`j2`|->`j3`,`m2`|->`m3`] 
+               (helperLib.MATCH_INST (SPEC_ALL move_list_thm) (concl th))))
+  \\ ASM_SIMP_TAC std_ss [] \\ REPEAT STRIP_TAC
+  \\ `CUT (i + n + 1,j) m = CUT (i + n + 1,j) m3` by ALL_TAC THEN1    
+    (FULL_SIMP_TAC std_ss [gc_inv_def,abs_gc_inv_def,LET_DEF]
+     \\ `!k. i + n + 1 <= k ==> b <= k` by DECIDE_TAC
+     \\ FULL_SIMP_TAC std_ss [FUN_EQ_THM,CUT_def,RANGE_def] \\ SET_TAC)
+  \\ `i + n + 1 <= j` by RANGE_TAC
+  \\ `D1 (CUT (i + n + 1,j) m3) UNION D1 (CUT (j,j3) m3) = D1 (CUT (i + n + 1,j3) m3)` 
+         by METIS_TAC [D1_UNION,gc_inv_def,abs_gc_inv_def] 
+  \\ FULL_SIMP_TAC std_ss [] \\ Q.LIST_EXISTS_TAC [`h3 |+ (i,ADDR_MAP f3 xs,n,d)`,`f3`]
+  \\ `~RANGE(b2,e2)i /\ RANGE(b,j3)i /\ RANGE(b,i+n+1)i` by RANGE_TAC
+  \\ FULL_SIMP_TAC std_ss [gc_inv_def,CUT_UPDATE] 
+  \\ ASM_SIMP_TAC std_ss [APPLY_UPDATE_THM]
+  \\ STRIP_TAC THEN1 RANGE_TAC \\ STRIP_TAC THEN1 METIS_TAC []
+  \\ `i IN D0 (CUT (b,i + n + 1) m3) /\  
+      (m3 i = H_BLOCK (xs,n,d))` by ALL_TAC THEN1
+     (`!k. k < i + n + 1 ==> k < j` by DECIDE_TAC
+      \\ FULL_SIMP_TAC std_ss [] 
+      \\ `CUT (b,i+n+1) m3 = CUT (b,i+n+1) m` by 
+          (FULL_SIMP_TAC std_ss [CUT_def,RANGE_def] \\ SET_TAC)
+      \\ `(CUT(b,i+n+1)m3) i = H_BLOCK (xs,n,d)` by ALL_TAC THEN1
+             (FULL_SIMP_TAC std_ss [] \\ FULL_SIMP_TAC std_ss [CUT_EQ,IN_DEF])
+      \\ FULL_SIMP_TAC std_ss [IN_DEF,D0,CUT_EQ,heap_element_11])
+  \\ FULL_SIMP_TAC std_ss [D0_UPDATE]  
+  \\ STRIP_TAC THEN1
+   (MATCH_MP_TAC (RW[AND_IMP_INTRO]full_heap_step)
+    \\ FULL_SIMP_TAC std_ss [APPLY_UPDATE_THM,heap_element_11,EMP_RANGE_def,IN_DEF]
+    \\ STRIP_TAC THEN1 METIS_TAC [full_heap_BLOCK]
+    \\ FULL_SIMP_TAC std_ss [CUT_def,FUN_EQ_THM] \\ REPEAT STRIP_TAC
+    \\ `RANGE (b,j) k /\ ~(RANGE (i + 1,i + n + 1) i)` by RANGE_TAC \\ SET_TAC)
+  \\ STRIP_TAC THEN1
+   (FULL_SIMP_TAC std_ss [IN_DEF,D0,CUT_EQ,heap_element_11]
+    \\ `~(i = j3)` by RANGE_TAC 
+    \\ METIS_TAC [full_heap_BLOCK,full_heap_cases,heap_element_11,PAIR_EQ])
+  \\ STRIP_TAC THEN1
+   (Q.EXISTS_TAC `len'` \\ ASM_SIMP_TAC std_ss []
+    \\ MATCH_MP_TAC part_heap_IGNORE \\ ASM_SIMP_TAC std_ss [])
+  \\ REPEAT STRIP_TAC THEN1
+   (FULL_SIMP_TAC std_ss [ref_mem_def,APPLY_UPDATE_THM,FDOM_FUPDATE,IN_INSERT]
+    \\ REPEAT STRIP_TAC \\ Cases_on `i = a` 
+    \\ FULL_SIMP_TAC std_ss [FAPPLY_FUPDATE_THM]) 
+  \\ MATCH_MP_TAC abs_steps_TRANS
+  \\ Q.EXISTS_TAC `(h3,D0 (CUT (b,i) m3),D0 (CUT (i,j3) m3),
+          D1 (CUT (i + n + 1,j3) m3),f3)` \\ ASM_SIMP_TAC std_ss []
+  \\ SIMP_TAC std_ss [abs_steps_def]
+  \\ MATCH_MP_TAC RTC_SINGLE
+  \\ SIMP_TAC std_ss [abs_step_cases] \\ DISJ2_TAC \\ DISJ1_TAC
+  \\ Q.LIST_EXISTS_TAC [`i`,`xs`,`(n,d)`] \\ ASM_SIMP_TAC std_ss []
+  \\ IMP_RES_TAC ok_heap_IMP \\ IMP_RES_TAC abs_steps_thm \\ POP_ASSUM (K ALL_TAC)
+  \\ `f3 o f3 = I` by FULL_SIMP_TAC std_ss [gc_inv_def,abs_gc_inv_def,LET_DEF]
+  \\ FULL_SIMP_TAC std_ss [SET_TRANSLATE_MAP,SET_TRANSLATE_def]
+  \\ Q.PAT_ASSUM `!a. bbb` (MP_TAC o Q.GEN `a` o Q.SPEC `(f3:num->num) a`)
+  \\ `!k. f3 (f3 k) = (k:num)` by FULL_SIMP_TAC std_ss [FUN_EQ_THM]
+  \\ FULL_SIMP_TAC std_ss [] \\ STRIP_TAC
+  \\ FULL_SIMP_TAC std_ss [SET_EQ_SUBSET,GSYM SUBSET_INSERT_DELETE,INSERT_SUBSET]
+  \\ SIMP_TAC std_ss [SUBSET_DEF,IN_INSERT,IN_DELETE] 
+  \\ `RANGE (i,j3) i` by RANGE_TAC
+  \\ ASM_SIMP_TAC std_ss [IN_DEF,D0,CUT_EQ,heap_element_11]
+  \\ REVERSE (REPEAT STRIP_TAC) 
+  THEN1 METIS_TAC [heap_element_distinct,ref_mem_def,heap_element_11,PAIR_EQ]
+  THEN1  
+   (FULL_SIMP_TAC std_ss [EMP_RANGE_def,IN_DEF,heap_element_11]
+    \\ CCONTR_TAC \\ FULL_SIMP_TAC std_ss []
+    \\ `RANGE(i+1,i+n+1)x /\ RANGE(b,j)x` by RANGE_TAC \\ RES_TAC
+    \\ FULL_SIMP_TAC std_ss [CUT_def,FUN_EQ_THM] \\ METIS_TAC [heap_element_distinct])  
+  THEN1 (FULL_SIMP_TAC std_ss [heap_element_11] \\ RANGE_TAC)
+  THEN1 (FULL_SIMP_TAC std_ss [heap_element_11] \\ RANGE_TAC)
+  THEN1 (FULL_SIMP_TAC std_ss [heap_element_11] \\ RANGE_TAC)
+  THEN1
+   (FULL_SIMP_TAC std_ss [heap_element_11] 
+    \\ REVERSE (Cases_on `RANGE(i+1,i+n+1)x`) THEN1 RANGE_TAC
+    \\ FULL_SIMP_TAC std_ss [EMP_RANGE_def,IN_DEF,heap_element_11]
+    \\ FULL_SIMP_TAC std_ss [CUT_def,FUN_EQ_THM]
+    \\ `m x = H_EMP` by SET_TAC
+    \\ `RANGE(b,j)x` by RANGE_TAC \\ RES_TAC
+    \\ FULL_SIMP_TAC std_ss [CUT_def,FUN_EQ_THM] \\ METIS_TAC [heap_element_distinct]));
+
+val gc_loop_thm = store_thm("gc_loop_thm",
+  ``!j h f m i2 m2.
+      gc_inv (h1,roots1,h,f) (b,i,j,e,b2,e2,m,D1(CUT(i,j)m)) ==>
+      (gc_loop (i,j,m) = (i2,m2)) ==>
+        ?h4 f4. gc_inv (h1,roots1,h4,f4) (b,i2,i2,e,b2,e2,m2,{}) /\ j <= i2 /\
+                !a. f a <> a ==> (f4 a = f a)``,
+  completeInduct_on `e - i` \\ NTAC 4 STRIP_TAC \\ Cases_on `i = j`
+  \\ ONCE_REWRITE_TAC [gc_loop_def] \\ ASM_SIMP_TAC std_ss [CUT_EMPTY] THEN1 SET_TAC
+  \\ NTAC 6 STRIP_TAC \\ `?i3 j3 m3. gc_step (i,j,m) = (i3,j3,m3)` by METIS_TAC [PAIR]
+  \\ FULL_SIMP_TAC std_ss [LET_DEF] \\ REPEAT STRIP_TAC \\ IMP_RES_TAC gc_step_thm    
+  \\ `(e - i3 < e - i) /\ (e - i3 = e - i3)`  by RANGE_TAC 
+  \\ RES_TAC \\ IMP_RES_TAC LESS_EQ_TRANS \\ ASM_SIMP_TAC std_ss [] \\ SET_TAC);
+
+val ok_full_heap_def = Define `
+  ok_full_heap (h,roots) (b,i,e,b2,e2,m) = 
+     b <= i /\ i <= e /\ b2 <= e2 /\ (e2 - b2 = e - b) /\ (~(e < b2) ==> e2 < b) /\
+     (!k. ~RANGE (b,i) k ==> (m k = H_EMP)) /\ 
+     (?t. part_heap b i m t) /\ ref_mem (h,I) m /\ ok_heap (h,roots)`;
+
+val ok_full_heap_IMP = store_thm("ok_full_heap_IMP",
+  ``ok_full_heap (h,roots) (b2,i,e2,b,e,m) ==>
+    gc_inv (h,roots,h,I) (b,b,b,e,b2,e2,m,ADDR_SET roots) /\
+    ADDR_SET roots SUBSET DR0 (CUT (b2,e2) m)``,
+  STRIP_TAC \\ FULL_SIMP_TAC std_ss [gc_inv_def,ok_full_heap_def,full_heap_REFL]
+  \\ IMP_RES_TAC ok_heap_IMP \\ REPEAT STRIP_TAC THEN1 RANGE_TAC  
+  \\ FULL_SIMP_TAC std_ss [CUT_EMPTY] 
+  THEN1 (Q.PAT_ASSUM `!k.bb` MATCH_MP_TAC \\ RANGE_TAC) 
+  THEN1 (`part_heap i e2 m 0` by ALL_TAC THEN1
+        (MATCH_MP_TAC part_heap_EMP_RANGE \\ FULL_SIMP_TAC std_ss [EMP_RANGE_def,IN_DEF]
+         \\ REPEAT STRIP_TAC \\ `~RANGE (b2,i) k` by RANGE_TAC \\ RES_TAC)
+      \\ IMP_RES_TAC part_heap_TRANS \\ Q.EXISTS_TAC `t` \\ FULL_SIMP_TAC std_ss []
+      \\ IMP_RES_TAC part_heap_LENGTH_LESS_EQ)
+  \\ SIMP_TAC std_ss [abs_steps_def,RTC_REFL]
+  \\ FULL_SIMP_TAC std_ss [ok_heap_def,UNION_SUBSET]
+  \\ FULL_SIMP_TAC std_ss [SUBSET_DEF] \\ REPEAT STRIP_TAC \\ RES_TAC
+  \\ SIMP_TAC std_ss [DR0,D0,R0,CUT_EQ,IN_DEF] \\ DISJ1_TAC
+  \\ `?x1 x2 x3. h ' x = (x1,x2,x3)` by METIS_TAC [PAIR]
+  \\ Cases_on `m x` \\ POP_ASSUM MP_TAC
+  \\ FULL_SIMP_TAC std_ss [ref_mem_def,heap_element_distinct]
+  \\ ONCE_REWRITE_TAC [EQ_SYM_EQ] \\ SIMP_TAC std_ss [heap_element_11]
+  \\ `RANGE (b2,i) x` by METIS_TAC [heap_element_distinct]
+  \\ REPEAT STRIP_TAC \\ RANGE_TAC);
+
+val full_heap_IMP_part_heap = store_thm("full_heap_IMP_part_heap",
+  ``!b e m. full_heap b e m ==> part_heap b e m (e-b)``,
+  HO_MATCH_MP_TAC full_heap_ind \\ REPEAT STRIP_TAC
+  THEN1 (SIMP_TAC std_ss [] \\ METIS_TAC [part_heap_cases])
+  \\ ONCE_REWRITE_TAC [part_heap_cases] \\ DISJ2_TAC \\ DISJ2_TAC 
+  \\ ASM_SIMP_TAC std_ss [CUT_EQ,heap_element_11]
+  \\ Q.EXISTS_TAC `e - (b + n + 1)` \\ ASM_SIMP_TAC std_ss [] 
+  \\ IMP_RES_TAC full_heap_LESS_EQ \\ DECIDE_TAC);
+
+val gc_thm = store_thm("gc_thm",
+  ``ok_full_heap (h,roots) (b2,i,e2,b,e,m) ==>
+    (gc (b2,e2,b,e,roots,m) = (b,i2,e,b2,e2,roots2,m2)) ==>
+    ?h2. ok_full_heap (h2,roots2) (b,i2,e,b2,e2,m2) /\ 
+         gc_exec (h,roots) (h2,roots2)``,
+  STRIP_TAC \\ IMP_RES_TAC ok_full_heap_IMP
+  \\ SIMP_TAC std_ss [gc_def,LET_DEF]
+  \\ `?r3 b3 m3. move_list (roots,b,m) = (r3,b3,m3)` by METIS_TAC [PAIR]
+  \\ `?i4 m4. gc_loop (b,b3,m3) = (i4,m4)` by METIS_TAC [PAIR] 
+  \\ ONCE_REWRITE_TAC [EQ_SYM_EQ] \\ ASM_SIMP_TAC std_ss [] \\ REPEAT STRIP_TAC
+  \\ IMP_RES_TAC (RW [UNION_EMPTY] (helperLib.SUBST_INST [``z:num set``|->``{}:num set``] move_list_thm))
+  \\ Q.PAT_ASSUM `gc_inv (h,roots,h3,f3) ttt` MP_TAC
+  \\ REPEAT (Q.PAT_ASSUM `gc_inv xxx yyy` (K ALL_TAC)) \\ STRIP_TAC
+  \\ IMP_RES_TAC gc_loop_thm 
+  \\ Q.PAT_ASSUM `r3 = ADDR_MAP f3 roots` MP_TAC
+  \\ REPEAT (Q.PAT_ASSUM `r3 = ADDR_MAP xx roots` (K ALL_TAC)) \\ STRIP_TAC
+  \\ FULL_SIMP_TAC std_ss []
+  \\ `f3 o f3 = I` by ALL_TAC THEN1
+      (FULL_SIMP_TAC std_ss [gc_inv_def]
+       \\ IMP_RES_TAC ok_heap_IMP \\ IMP_RES_TAC abs_steps_thm 
+       \\ FULL_SIMP_TAC std_ss [abs_gc_inv_def,LET_DEF,gc_inv_def])
+  \\ Q.PAT_ASSUM `gc_inv (h,roots,h4,f4) ttt` MP_TAC
+  \\ REPEAT (Q.PAT_ASSUM `gc_inv xxx yyy` (K ALL_TAC))
+  \\ SIMP_TAC std_ss [gc_inv_def] \\ REPEAT STRIP_TAC 
+  \\ Q.EXISTS_TAC `DRESTRICT h4 (D0 (CUT (b,i4) m4))`
+  \\ FULL_SIMP_TAC std_ss [CUT_EMPTY] \\ helperLib.CLEAN_TAC
+  \\ `gc_exec (h,roots) (DRESTRICT h4 (D0 (CUT (b,i4) m4)),ADDR_MAP f3 roots)` by 
+      (MATCH_MP_TAC abs_gc_thm \\ ASM_SIMP_TAC std_ss []   
+       \\ SIMP_TAC std_ss [abs_gc_cases] 
+       \\ Q.LIST_EXISTS_TAC [`h4`,`f4`,`(D0 (CUT (b,i4) m4))`]
+       \\ ASM_SIMP_TAC std_ss [ADDR_MAP_EQ_ADDR_MAP]
+       \\ FULL_SIMP_TAC std_ss [SET_TRANSLATE_MAP,SET_TRANSLATE_def]
+       \\ FULL_SIMP_TAC std_ss [FUN_EQ_THM] \\ SET_TAC)
+  \\ IMP_RES_TAC gc_exec_thm
+  \\ ASM_SIMP_TAC std_ss []
+  \\ FULL_SIMP_TAC std_ss [ok_full_heap_def] \\ REPEAT STRIP_TAC
+  THEN1 RANGE_TAC THEN1 FULL_SIMP_TAC std_ss [CUT_def,IN_DEF]
+  THEN1 METIS_TAC [full_heap_IMP_part_heap,EQ_RANGE_full_heap,EQ_RANGE_CUT]
+  \\ FULL_SIMP_TAC std_ss [ref_mem_def,FUN_EQ_THM,FDOM_DRESTRICT,IN_INTER]
+  \\ ASM_SIMP_TAC std_ss [IN_DEF,D0,CUT_EQ]
+  \\ REPEAT STRIP_TAC \\ CONV_TAC (RATOR_CONV (ONCE_REWRITE_CONV [CUT_def]))
+  \\ Cases_on `RANGE (b,i4) a` \\ ASM_SIMP_TAC std_ss [IN_DEF]
+  \\ Cases_on `FDOM h4 a` \\ ASM_SIMP_TAC std_ss [IN_DEF] THEN1
+     (`?x1 x2 x3. h4 ' a = (x1,x2,x3)` by METIS_TAC [PAIR]
+      \\ ASM_SIMP_TAC std_ss [heap_element_11,DRESTRICT_DEF,IN_INTER]
+      \\ FULL_SIMP_TAC std_ss [IN_DEF,D0,CUT_EQ,heap_element_11])
+  \\ Cases_on `f4 a = a` \\ ASM_SIMP_TAC std_ss [heap_element_distinct]
+  \\ FULL_SIMP_TAC std_ss [abs_gc_inv_def,LET_DEF,NOT_IN_EMPTY,IN_UNION]      
+  \\ FULL_SIMP_TAC std_ss [FUN_EQ_THM]   
+  \\ `R0 m4 a` by FULL_SIMP_TAC std_ss [R0,IN_DEF,heap_element_11]
+  \\ METIS_TAC [full_heap_R0]);
+
+val _ = export_theory();
